coq_alt/Ltms.v
@@ -1,0 +1,3107 @@
+Set Implicit Arguments.
+Require Import Strings.String Strings.Ascii Numbers.Natural.Peano.NPeano Lists.List Program.Equality Recdef.
+Require Import CSC.Sets CSC.Util CSC.Fresh CSC.Props.
+
+From RecordUpdate Require Import RecordSet.
+
+
+(** * Syntax *)
+
+(** These are the locs from the L³ paper by Ahmed, Fluet, and Morrisett *)
+Inductive Loc : Type :=
+| LConst : loc -> Loc
+| LVar : vart -> Loc
+.
+Definition Loc_eqb (l1 l2 : Loc) : bool :=
+  match l1, l2 with
+  | LConst l1, LConst l2 => (l1 == l2)
+  | LVar v1, LVar v2 => (v1 == v2)
+  | _, _ => false
+  end
+.
+Lemma Loc_eqb_eq l0 l1 :
+  Loc_eqb l0 l1 = true <-> l0 = l1.
+Proof.
+  split; intros H; destruct l0, l1; cbn in *; try easy;
+  try ((change ((l == l0) = true) in H + change ((v == v0) = true) in H);
+       apply eqb_eq in H; subst; easy).
+  inv H; change ((l0 == l0) = true); apply eq_refl.
+  inv H; change ((v0 == v0) = true); apply eq_refl.
+Qed.
+#[local]
+Instance Loceq__Instance : HasEquality Loc := {
+  eq := Loc_eqb ;
+  eqb_eq := Loc_eqb_eq ;
+}.
+(** Values are numbers, pairs, capabilities, and pointers *)
+Inductive value : Type :=
+| Vnat : nat -> value
+| Vpair : value -> value -> value
+| Vcap : value
+| Vptr : loc -> value
+| Vpack : Loc -> value -> value
+.
+Coercion Vnat : nat >-> value.
+Fixpoint value_eqb (v1 v2 : value) : bool :=
+  match v1, v2 with
+  | Vnat n1, Vnat n2 => Nat.eqb n1 n2
+  | Vpair v0 v1, Vpair v0' v1' => andb (value_eqb v0 v0') (value_eqb v1 v1')
+  | Vcap, Vcap => true
+  | Vptr l0, Vptr l1 => l0 == l1
+  | Vpack l0 v0, Vpack l1 v1 => andb (l0 == l1) (value_eqb v0 v1)
+  | _, _ => false
+  end
+.
+Lemma value_eqb_eq v1 v2 :
+  value_eqb v1 v2 = true <-> v1 = v2.
+Proof.
+  revert v2; induction v1; cbn; split; intros.
+  - destruct v2; try easy. apply Nat.eqb_eq in H; inv H; reflexivity.
+  - destruct v2; inv H; apply Nat.eqb_refl.
+  - destruct v2; inv H. eq_to_defeq value_eqb. apply IHv1_1 in H; apply IHv1_2 in H0.
+    subst. reflexivity.
+  - inv H; cbn. eq_to_defeq value_eqb; split. now apply IHv1_1. now apply IHv1_2.
+  - destruct v2; inv H. reflexivity.
+  - destruct v2; inv H. reflexivity.
+  - destruct v2; inv H; eq_to_defeq loc_eqb.
+  - destruct v2; inv H; eq_to_defeq loc_eqb.
+  - destruct v2; inv H; eq_to_defeq Loc_eqb. apply IHv1 in H0; subst. reflexivity.
+  - destruct v2; inv H; eq_to_defeq Loc_eqb; split; try easy. now apply IHv1.
+Qed.
+#[local]
+Instance valueeq__Instance : HasEquality value := {
+  eq := value_eqb ;
+  eqb_eq := value_eqb_eq ;
+}.
+#[local]
+Existing Instance varteq__Instance.
+(** Possible binary operations. *)
+Variant binopsymb : Type :=
+| Badd : binopsymb
+| Bsub : binopsymb
+| Bmul : binopsymb
+| Bdiv : binopsymb
+| Bless : binopsymb
+.
+#[local]
+Existing Instance varteq__Instance.
+Inductive expr : Type :=
+| Xval (v : value) : expr
+| Xvar (x : vart) : expr
+| Xbinop (symb : binopsymb) (lhs rhs : expr) : expr
+| Xget (e0 e1 e2 : expr) : expr
+| Xset (e0 e1 e2 e3 : expr) : expr
+| Xlet (x : vart) (e0 e1 : expr) : expr
+| Xnew (e : expr) : expr
+| Xdel (e : expr) : expr
+| Xunpack (γ x : vart) (e0 e1 : expr) : expr
+| Xpack (ℓ : Loc) (e : expr) : expr
+| Xpair (e1 e2 : expr) : expr
+| Xunpair (x1 x2 : vart) (e1 e2 : expr) : expr
+| Xreturn (e : expr) : expr
+| Xcall (foo : vart) (e : expr) : expr
+| Xifz (c e0 e1 : expr) : expr
+| Xabort : expr
+.
+(** The following is a helper function to easily define functions over the syntax of S, e.g. substitution. *)
+Definition exprmap (h : expr -> expr) (e : expr) :=
+  match e with
+  | Xbinop b lhs rhs => Xbinop b (h lhs) (h rhs)
+  | Xget e0 e1 e2 => Xget (h e0) (h e1) (h e2)
+  | Xset e0 e1 e2 e3 => Xset (h e0) (h e1) (h e2) (h e3)
+  | Xlet x e0 e1 => Xlet x (h e0) (h e1)
+  | Xnew e => Xnew (h e)
+  | Xdel e => Xdel (h e)
+  | Xunpack x ℓ e0 e1 => Xunpack x ℓ (h e0) (h e1)
+  | Xpack ℓ e => Xpack ℓ (h e)
+  | Xpair e1 e2 => Xpair (h e1) (h e2)
+  | Xunpair x1 x2 e1 e2 => Xunpair x1 x2 (h e1) (h e2)
+  | Xreturn e => Xreturn (h e)
+  | Xcall f e => Xcall f (h e)
+  | Xifz c e0 e1 => Xifz (h c) (h e0) (h e1)
+  | _ => e
+  end
+.
+(** We proceed to define the dynamic semantics via evaluation contexts/environments. *)
+Inductive evalctx : Type :=
+| Khole : evalctx
+| KbinopL (b : binopsymb) (K : evalctx) (e : expr) : evalctx
+| KbinopR (b : binopsymb) (v : value) (K : evalctx) : evalctx
+| KgetL (K : evalctx) (e0 e1 : expr) : evalctx
+| KgetM (v : value) (K : evalctx) (e1 : expr) : evalctx
+| KgetR (v0 v1 : value) (K : evalctx) : evalctx
+| KsetL (K : evalctx) (e0 e1 e2 : expr) : evalctx
+| KsetM0 (v : value) (K : evalctx) (e0 e1 : expr) : evalctx
+| KsetM1 (v0 v1 : value) (K : evalctx) (e : expr) : evalctx
+| KsetR (v0 v1 v2 : value) (K : evalctx) : evalctx
+| Klet (x : vart) (K : evalctx) (e : expr) : evalctx
+| Knew (K : evalctx) : evalctx
+| Kdel (K : evalctx) : evalctx
+| Kunpack (γ x : vart) (K : evalctx) (e : expr) : evalctx
+| Kpack (ℓ : Loc) (K : evalctx) : evalctx
+| KpairL (K : evalctx) (e : expr) : evalctx
+| KpairR (v : value) (K : evalctx) : evalctx
+| Kunpair (x1 x2 : vart) (K : evalctx) (e : expr) : evalctx
+| Kifz (K : evalctx) (e0 e1 : expr) : evalctx
+| Kreturn (K : evalctx) : evalctx
+| Kcall (foo : vart) (K : evalctx) : evalctx
+.
+(** Pre-Types of S *)
+Inductive pre_ty : Type :=
+| Tnat : pre_ty
+| Tptr : Loc -> pre_ty
+| Tcap : Loc -> pre_ty -> pre_ty
+| Tpair : pre_ty -> pre_ty -> pre_ty
+| Texists : vart -> pre_ty -> pre_ty
+.
+Notation "'Tℕ'" := (Tnat).
+Fixpoint pre_ty_eqb (t1 t2 : pre_ty) : bool :=
+  match t1, t2 with
+  | Tnat, Tnat => true
+  | Tptr l1, Tptr l2 => (l1 == l2)
+  | Tcap l1 t1, Tcap l2 t2 => andb (l1 == l2) (pre_ty_eqb t1 t2)
+  | Tpair t1 t2, Tpair t1' t2' => andb (pre_ty_eqb t1 t1') (pre_ty_eqb t2 t2')
+  | Texists x t1, Texists y t2 => andb (x == y) (pre_ty_eqb t1 t2)
+  | _, _ => false
+  end
+.
+Lemma pre_ty_eqb_eq t0 t1 :
+  pre_ty_eqb t0 t1 = true <-> t0 = t1.
+Proof.
+  split; revert t1; induction t0; intros.
+  - destruct t1; now cbn.
+  - destruct t1; cbn in H; try easy. eq_to_defeq Loc_eqb.
+  - destruct t1; cbn in H; try easy. eq_to_defeq Loc_eqb.
+    specialize (IHt0 t1 H0); subst; reflexivity.
+  - destruct t1; cbn in H; try easy. eq_to_defeq pre_ty_eqb.
+    specialize (IHt0_1 t1_1 H); specialize (IHt0_2 t1_2 H0); subst.
+    reflexivity.
+  - destruct t1; cbn in H; try easy. eq_to_defeq vareq.
+    specialize (IHt0 t1 H0); subst; reflexivity.
+  - now destruct t1.
+  - destruct t1; try easy; inv H; cbn; eq_to_defeq Loc_eqb.
+  - destruct t1; try easy; inv H; cbn; eq_to_defeq Loc_eqb.
+    split; eq_to_defeq Loc_eqb. eapply IHt0; eauto.
+  - destruct t1; inv H. cbn; eq_to_defeq eq. split; eauto.
+  - destruct t1; try easy; inv H; cbn; eq_to_defeq vareq; split;
+    eq_to_defeq vareq; eapply IHt0; eauto.
+Qed.
+#[local]
+Instance pre_tyeq__Instance : HasEquality pre_ty := {
+  eq := pre_ty_eqb ;
+  eqb_eq := pre_ty_eqb_eq ;
+}.
+#[local]
+Existing Instance varteq__Instance.
+
+(** Types of S *)
+Inductive ty : Type :=
+| Tpre : pre_ty -> ty
+| Tret : pre_ty -> ty
+| Tfun : pre_ty -> pre_ty -> ty
+.
+Definition ty_eqb (t1 t2 : ty) : bool :=
+  match t1, t2 with
+  | Tpre t1, Tpre t2 => (t1 == t2)
+  | Tret t1, Tret t2 => (t1 == t2)
+  | Tfun t1 t2, Tfun t1' t2' => andb (t1 == t1') (t2 == t2')
+  | _, _ => false
+  end
+.
+Lemma ty_eqb_eq t0 t1 :
+  ty_eqb t0 t1 = true <-> t0 = t1.
+Proof.
+  destruct t0, t1; split; intros H; try easy; cbn in H;
+  eq_to_defeq pre_ty_eqb; inv H; cbn; eq_to_defeq pre_ty_eqb.
+Qed.
+#[local]
+Instance tyeq__Instance : HasEquality ty := {
+  eq := ty_eqb ;
+  eqb_eq := ty_eqb_eq ;
+}.
+#[local]
+Existing Instance varteq__Instance.
+
+(** Static Environments. Value Contexts and Location Contexts *)
+Definition Gamma : Type := mapind varteq__Instance ty.
+Definition Delta : Type := list vart.
+
+(** Interface types. These are the only things allowed to be passed
+    across the boundary, i.e., context to comp (!) or vice versa (?). *)
+Inductive int : ty -> Prop :=
+| intℕ : int (Tpre Tℕ)
+.
+Definition intf (τ : ty) : option ty :=
+  match τ with
+  | Tpre Tℕ => Some(Tpre Tℕ)
+  | _ => None
+  end
+.
+Lemma intf_refl τ τ' :
+  intf τ = Some τ' -> τ = τ'.
+Proof. induction τ; cbn; intros; inv H; try easy. destruct p; try easy. now inv H1. Qed.
+Lemma int_equiv_intf τ :
+  int τ <-> intf τ = Some τ
+.
+Proof.
+  destruct τ; cbn; try easy.
+  now induction p; cbn.
+Qed.
+Ltac crush_intf τ :=
+  let Hx' := fresh "Hx'" in
+  let Hx := fresh "Hx" in
+  let x := fresh "x" in
+  destruct (option_dec (intf τ)) as [Hx | Hx];
+  try (rewrite Hx in *; congruence);
+  try (apply not_eq_None_Some in Hx as [x Hx]; eapply intf_refl in Hx as Hx'; rewrite <- Hx' in Hx; clear Hx'; rewrite Hx in *)
+.
+Lemma int_equiv_intf_none τ :
+  (~ int τ) <-> intf τ = None
+.
+Proof.
+  split; intros H.
+  - crush_intf τ; apply int_equiv_intf in Hx; contradiction.
+  - intros H0%int_equiv_intf; congruence.
+Qed.
+
+(** Symbols look like `fn foo x : τ := e` *)
+Definition symbol : Type := vart * ty * expr.
+Definition symbols := mapind varteq__Instance symbol.
+
+Definition vart_of_symbol (s : symbol) := let '(v, t, e) := s in v.
+Definition expr_of_symbol (s : symbol) := let '(v, t, e) := s in e.
+Definition ty_of_symbol (s : symbol) := let '(v, t, e) := s in t.
+
+(** Type for list of relevant functions, i.e. those that are part of the component. *)
+Definition commlib := list vart.
+
+(** A program is just a collection of context and of component symbols.
+    The symbol `main` is the associated entry-point. *)
+Inductive prog : Type := Cprog : symbols -> symbols -> prog.
+
+
+Definition string_of_prog (p : prog) :=
+  let '(Cprog Ξ__ctx Ξ__comp) := p in
+  "prog"%string (*TODO*)
+.
+(** Fill hole in evaluation context. *)
+Fixpoint insert (K : evalctx) (withh : expr) : expr :=
+  let R := fun k => insert k withh in
+  match K with
+  | Khole => withh
+  | KbinopL b K' e => Xbinop b (R K') e
+  | KbinopR b v K' => Xbinop b (Xval v) (R K')
+  | KgetL K' e0 e1 => Xget (R K') e0 e1
+  | KgetM v K' e => Xget (Xval v) (R K') e
+  | KgetR v0 v1 K' => Xget (Xval v0) (Xval v1) (R K')
+  | KsetL K' e0 e1 e2 => Xset (R K') e0 e1 e2
+  | KsetM0 v K' e0 e1 => Xset (Xval v) (R K') e0 e1
+  | KsetM1 v0 v1 K' e => Xset (Xval v0) (Xval v1) (R K') e
+  | KsetR v0 v1 v2 K' => Xset (Xval v0) (Xval v1) (Xval v2) (R K')
+  | Klet x K' e => Xlet x (R K') e
+  | Knew K' => Xnew (R K')
+  | Kdel K' => Xdel (R K')
+  | Kunpack γ x K' e => Xunpack γ x (R K') e
+  | Kpack ℓ K' => Xpack ℓ (R K')
+  | KpairL K' e => Xpair (R K') e
+  | KpairR v K' => Xpair (Xval v) (R K')
+  | Kunpair x1 x2 K' e => Xunpair x1 x2 (R K') e
+  | Kifz K' e0 e1 => Xifz (R K') e0 e1
+  | Kreturn K' => Xreturn (R K')
+  | Kcall foo K' => Xcall foo (R K')
+  end
+.
+
+(** Simple projection giving us the names of the symbols *)
+Fixpoint interfaces (s : symbols) : option(Gamma) :=
+  match s with
+  | mapNil _ _ => Some (mapNil _ _)
+  | mapCons name EL s' =>
+    let ty := ty_of_symbol EL in
+    let name := vart_of_symbol EL in
+    let* a := interfaces s' in
+    Some(name ↦ ty ◘ a)
+  end
+.
+
+(** * Dynamics *)
+
+(** Evaluation of binary expressions. Note that 0 means `true` in S, so `5 < 42` evals to `0`. *)
+Definition eval_binop (b : binopsymb) (v0 v1 : value) : option value :=
+  let* n0 := match v0 with | Vnat n => Some n | _ => None end in
+  let* n1 := match v1 with | Vnat n => Some n | _ => None end in
+  Some(Vnat(match b with
+       | Bless => (if Nat.ltb n0 n1 then 0 else 1)
+       | Badd => (n0 + n1)
+       | Bdiv => (n0 / n1)
+       | Bsub => (n0 - n1)
+       | Bmul => (n0 * n1)
+       end))
+.
+(** Poison used to mark locations in our operational state. *)
+Inductive poison : Type :=
+| poisonless : poison
+| poisoned : poison
+.
+Notation "'◻'" := (poisonless).
+Notation "'☣'" := (poisoned).
+Definition poison_eqb :=
+  fun (ρ1 ρ2 : poison) =>
+    match ρ1, ρ2 with
+    | ◻, ◻ | ☣, ☣ => true
+    | _, _ => false
+    end
+.
+Lemma poison_eqb_eq ρ1 ρ2 :
+  poison_eqb ρ1 ρ2 = true <-> ρ1 = ρ2.
+Proof. destruct ρ1, ρ2; now cbn. Qed.
+#[local]
+Instance poisoneq__Instance : HasEquality poison := {
+  eq := poison_eqb ;
+  eqb_eq := poison_eqb_eq ;
+}.
+
+(* A "dynamic" location contains the location and its poison *)
+Record dynloc : Type := {
+  dℓ : loc ;        (* concrete location on heap *)
+  dρ : poison ;     (* wether the location is already deallocated *)
+  dt : ControlTag ; (* which heap the data lies on  *)
+  dn : nat ;          (* allocation size *)
+}.
+Definition dynloc_eqb :=
+  fun (dℓ1 dℓ2 : dynloc) =>
+    andb  (dℓ1.(dℓ) == dℓ2.(dℓ))
+    (andb (dℓ1.(dρ) == dℓ2.(dρ))
+    (andb (dℓ1.(dt) == dℓ2.(dt))
+          (Nat.eqb dℓ1.(dn) dℓ2.(dn))))
+.
+Lemma dynloc_eqb_eq dℓ0 dℓ1 :
+  dynloc_eqb dℓ0 dℓ1 = true <-> dℓ0 = dℓ1.
+Proof.
+  unfold dynloc_eqb; split; intros.
+  eq_to_defeq Nat.eqb. apply Nat.eqb_eq in H2. cbv in *; destruct dℓ0, dℓ1; inv H; inv H3; reflexivity.
+  inv H; eq_to_defeq Nat.eqb; try apply Nat.eqb_eq. repeat split; try apply eq_refl. apply Nat.eqb_refl.
+Qed.
+#[local]
+Instance dynloceq__Instance : HasEquality dynloc := {
+  eq := dynloc_eqb ;
+  eqb_eq := dynloc_eqb_eq ;
+}.
+Notation "'dL(' bℓ ';' bρ ';' bt ';' bn ')'" := (({| dℓ := bℓ ;
+                                                     dρ := bρ ;
+                                                     dt := bt ;
+                                                     dn := bn |}) : dynloc) (at level 80).
+(** Stores map variables to potentially poisoned locations. *)
+Definition store := mapind varteq__Instance dynloc.
+Definition sNil : store := mapNil varteq__Instance dynloc.
+
+(** Stores pointers and their respective metadata. *)
+Definition ptrstore := mapind loceq__Instance dynloc.
+Definition snil : ptrstore := mapNil loceq__Instance dynloc.
+
+Fixpoint δ_of_Δ (Δ : store) :=
+  match Δ with
+  | mapNil _ _ => mapNil _ _
+  | mapCons _ ddℓ Δ' => let '(addr a) := ddℓ.(dℓ) in mapCons (addr a) (Util.addr a) (δ_of_Δ Δ')
+  end
+.
+
+Inductive snodupinv : store -> Prop :=
+| snodupmapNil : snodupinv (sNil)
+| snodupmapCons : forall (x : vart) (ℓ : loc) (ρ : poison) (t : ControlTag) (n : nat) (Δ : store),
+    ~(List.In x (dom Δ)) ->
+    ~(List.In ℓ (dom(δ_of_Δ Δ))) ->
+    snodupinv Δ ->
+    snodupinv (x ↦ dL(ℓ ; ρ ; t ; n) ◘ Δ)
+.
+Lemma nodupinv_of_snodupinv (Δ : store) :
+  snodupinv Δ ->
+  nodupinv Δ
+.
+Proof. induction 1; constructor; eauto. Qed.
+
+Fixpoint sundup (Δ : store) : option(store) :=
+  match Δ with
+  | mapNil _ _ => Some(mapNil _ _)
+  | mapCons a ddℓ Δ' =>
+    let thedom := dom Δ' in
+    let theimg := img Δ' in
+    match List.find (fun x => eq a x) thedom, List.find (fun x => loc_eqb x.(dℓ) ddℓ.(dℓ)) theimg, sundup Δ' with
+    | None, None, Some Δ'' => Some(mapCons a ddℓ Δ'')
+    | _, _, _ => None
+    end
+  end
+.
+Lemma sundup_refl (Δ Δ' : store) :
+  sundup Δ = Some Δ' -> Δ = Δ'.
+Proof.
+  revert Δ'; induction Δ; cbn; intros; try (inv H; easy).
+  destruct b. destruct (option_dec (List.find (fun x : vart => vareq a x) (dom Δ))) as [Hx|Hy].
+  - apply not_eq_None_Some in Hx as [Δ__x Hx]; rewrite Hx in H; congruence.
+  - rewrite Hy in H.
+    cbn in H. crush_option (List.find (fun x => loc_eqb (dℓ x) dℓ0) (img Δ)).
+    + inv H.
+    + rewrite Hx in H. destruct (option_dec (sundup Δ)) as [Hx1|Hy1].
+      * apply not_eq_None_Some in Hx1 as [Δ__x Hx1]; rewrite Hx1 in H.
+        specialize (IHΔ Δ__x Hx1) as ->; now inv H.
+      * rewrite Hy1 in H; congruence.
+Qed.
+Lemma δ_of_Δ_in_dom (Δ : store) ℓ :
+  In ℓ (dom (δ_of_Δ Δ)) ->
+  exists ρ t n, In (dL(ℓ ; ρ ; t ; n)) (img Δ)
+.
+Proof.
+  revert ℓ; induction Δ; cbn; intros; try easy.
+  destruct b, dℓ0; destruct H as [H|H].
+  - inv H. exists dρ0; exists dt0; exists dn0; now left.
+  - specialize (IHΔ ℓ H); deex; exists ρ; exists t; exists n0; now right.
+Qed.
+Lemma δ_of_Δ_in_img (Δ : store) ℓ ρ t n :
+  In (dL(ℓ ; ρ ; t ; n)) (img Δ) ->
+  In ℓ (dom (δ_of_Δ Δ))
+.
+Proof.
+  induction Δ; cbn; intros H; try easy.
+  destruct H as [H|H]; destruct b, dℓ0.
+  - inv H. now left.
+  - specialize (IHΔ H). now right.
+Qed.
+Lemma snodupinv_equiv_sundup (Δ : store) :
+  sundup Δ = Some Δ <-> snodupinv Δ.
+Proof.
+  split; intros H.
+  - induction Δ; cbn; try constructor.
+    cbn in H. destruct b. destruct (option_dec (List.find (fun x : vart => vareq a x) (dom Δ))) as [Hx|Hy].
+    + apply not_eq_None_Some in Hx as [Δ__x Hx]; rewrite Hx in H; congruence.
+    + rewrite Hy in H. cbn in H. destruct (option_dec (List.find (fun x => loc_eqb (dℓ x) dℓ0) (img Δ))) as [Hx0|Hy0].
+      * apply not_eq_None_Some in Hx0 as [Δ__x0 Hx0]; rewrite Hx0 in H; congruence.
+      * rewrite Hy0 in H. destruct (option_dec (sundup Δ)) as [Hx1|Hy1].
+        -- apply not_eq_None_Some in Hx1 as [Δ__x Hx1]; rewrite Hx1 in H.
+           rewrite <- (sundup_refl _ Hx1) in Hx1. specialize (IHΔ Hx1).
+           econstructor; eauto.
+           intros H__a. eapply find_none in Hy as Hy__f; eauto. unfold vareq in Hy__f.
+           now rewrite String.eqb_refl in Hy__f.
+           intros H__a.
+           apply δ_of_Δ_in_dom in H__a as H__a'; deex.
+           eapply find_none in Hy0 as Hy0__f; eauto; cbn in Hy0__f; eq_to_defeq loc_eqb. apply neqb_neq in Hy0__f. congruence.
+        -- rewrite Hy1 in H; congruence.
+  - induction H; cbn; try easy.
+    destruct (option_dec (List.find (fun x0 : vart => vareq x x0) (dom Δ))) as [Hx|Hy].
+    + apply not_eq_None_Some in Hx as [x__x Hx].
+      apply find_some in Hx as [Hx1 Hx2]. unfold vareq in Hx2. apply String.eqb_eq in Hx2; subst. contradiction.
+    + rewrite Hy. destruct (option_dec (List.find (fun x => loc_eqb (dℓ x) ℓ) (img Δ))) as [Hx0|Hy0].
+      * apply not_eq_None_Some in Hx0 as [[ℓ__x ρ__x] Hx0].
+        apply find_some in Hx0 as [Hx1 Hx2]. apply loc_eqb_eq in Hx2; subst.
+        apply δ_of_Δ_in_img in Hx1. contradiction.
+      * rewrite Hy0. rewrite IHsnodupinv. easy.
+Qed.
+Definition spush (x : vart) (dℓ : dynloc) (Δ : store) : option (store) :=
+  match sundup (mapCons x dℓ Δ) with
+  | Some Δ' => Some Δ'
+  | None => None
+  end
+.
+Lemma spush_ok (x : vart) (dℓ : dynloc) (Δ Δ' : store) :
+  spush x dℓ Δ = Some Δ' -> snodupinv Δ'.
+Proof.
+  intros H0. unfold spush in H0.
+  destruct (option_dec (sundup (mapCons x dℓ Δ))) as [Hx|Hy]; try (rewrite Hy in *; congruence);
+  apply not_eq_None_Some in Hx as [Δ__x Hx]; rewrite Hx in H0; inv H0;
+  apply snodupinv_equiv_sundup; cbn in Hx.
+  destruct dℓ.
+  destruct (option_dec (List.find (fun x0 : vart => vareq x x0) (dom Δ))) as [Hx0|Hy0]; try (rewrite Hy0 in *; congruence).
+  apply not_eq_None_Some in Hx0 as [Δ__x Hx0]; rewrite Hx0 in Hx; inv Hx.
+  rewrite Hy0 in Hx. cbn in Hx. destruct (option_dec (List.find (fun x => loc_eqb (dℓ x) dℓ0) (img Δ))) as [Hx1|Hy1].
+  apply not_eq_None_Some in Hx1 as [Δ__x Hx1]; rewrite Hx1 in Hx; inv Hx.
+  rewrite Hy1 in Hx. destruct (option_dec (sundup Δ)) as [Hx2|Hy2].
+  apply not_eq_None_Some in Hx2 as [Δ__x Hx1]. rewrite Hx1 in Hx.
+  inv Hx. cbn. apply sundup_refl in Hx1 as Hx1'. rewrite Hx1' in Hy0.
+  rewrite (sundup_refl Δ Hx1) in Hx1. rewrite Hx1' in Hy1. rewrite Hy0, Hy1, Hx1; easy.
+  rewrite Hy2 in Hx; congruence.
+Qed.
+Lemma snodupinv_whocares0 (a : vart) (ℓ : loc) (ρ ρ' : poison) (t t' : ControlTag) (n n' : nat) (Δ : store) :
+  snodupinv (a ↦ (dL(ℓ ; ρ ; t ; n)) ◘ Δ) <-> snodupinv (a ↦ (dL(ℓ ; ρ' ; t' ; n')) ◘ Δ)
+.
+Proof. split; intros H; constructor; inv H; eauto. Qed.
+Lemma snodupinv_split (Δ Δ' : store) :
+  snodupinv (Δ ◘ Δ') ->
+  snodupinv Δ /\ snodupinv Δ'
+.
+Proof.
+  remember (Δ ◘ Δ') as Δ__c; revert Δ Δ' HeqΔ__c; induction Δ__c; cbn; intros.
+  - now destruct Δ, Δ'; inv HeqΔ__c.
+  - destruct Δ, Δ'; inv HeqΔ__c; cbn in *.
+    + split; try constructor; easy.
+    + split; try constructor; now rewrite append_nil in H.
+    + inv H. specialize (IHΔ__c Δ (v0 ↦ d0 ◘ Δ') Logic.eq_refl H5) as [IH__a IH__b].
+      split; try easy.
+      constructor; try easy.
+      * revert H3; clear; intros H0 H1; induction Δ; inv H1.
+        apply H0; now left.
+        assert (~ In v (dom (Δ ◘ v0 ↦ d0 ◘ Δ'))) as H2 by (intros H2; apply H0; now right); auto.
+      * revert H4; clear; intros H0 H1; induction Δ; try inv H1.
+        cbn in H1; destruct b, dℓ0; inv H1. apply H0; now left.
+        assert (~ In ℓ (dom(δ_of_Δ (Δ ◘ v0 ↦ d0 ◘ Δ')))) as H2 by (intros H2; apply H0; now right); auto.
+Qed.
+
+Lemma snodupinv_whocares (a : vart) (ℓ : loc) (ρ ρ' : poison) (t t' : ControlTag) (n n' : nat) (Δ Δ' : store) :
+  snodupinv (Δ ◘ a ↦ (dL(ℓ ; ρ ; t ; n)) ◘ Δ') <-> snodupinv (Δ ◘ a ↦ (dL(ℓ ; ρ' ; t' ; n')) ◘ Δ')
+.
+Proof.
+Admitted.
+Lemma spush_msubset (Δ Δ' : store) (x : vart) (v : dynloc) :
+  Some Δ' = spush x v Δ ->
+  MSubset Δ Δ'.
+Proof. Admitted.
+
+Lemma δΔ_msubset_invariant (Δ Δ' : store) :
+  MSubset Δ Δ' ->
+  MSubset (δ_of_Δ Δ) (δ_of_Δ Δ')
+.
+Proof. Admitted.
+
+#[local]
+Instance nateq__Instance : HasEquality nat := {
+  eq := Nat.eqb ;
+  eqb_eq := Nat.eqb_eq ;
+}.
+Definition heap := mapind nateq__Instance (option value).
+Definition hNil : heap := mapNil nateq__Instance (option value).
+Fixpoint Hgrow_aux (H : heap) (s len : nat) : option heap :=
+  match s with
+  | 0 => Some(H)
+  | S n' =>
+    let* Hi := Hgrow_aux H n' len in
+    push (len + n') None Hi
+  end
+.
+Definition Hgrow (H : heap) (s : nat) : option heap :=
+  Hgrow_aux H s (List.length (dom H))
+.
+(* Context switch indicators. The paper calls these Transfer Tags *)
+Variant comms : Type :=
+| Qctxtocomp : comms
+| Qcomptoctx : comms
+| Qinternal : comms
+.
+Definition comms_eqb (q1 q2 : comms) :=
+  match q1, q2 with
+  | Qctxtocomp, Qctxtocomp => true
+  | Qcomptoctx, Qcomptoctx => true
+  | Qinternal, Qinternal => true
+  | _, _ => false
+  end
+.
+Lemma comms_eqb_eq (q1 q2 : comms) :
+  comms_eqb q1 q2 = true <-> q1 = q2.
+Proof.
+  destruct q1, q2; now cbn.
+Qed.
+#[local]
+Instance commseq__Instance : HasEquality comms := {
+  eq := comms_eqb ;
+  eqb_eq := comms_eqb_eq ;
+}.
+Definition string_of_comms (q : comms) :=
+  match q with
+  | Qctxtocomp => "?"%string
+  | Qcomptoctx => "!"%string
+  | Qinternal => "∅"%string
+  end
+.
+(* Continuation Stacks *)
+Definition active_ectx := list (evalctx * vart).
+
+#[local]
+Existing Instance varteq__Instance | 0.
+Record CfState : Type := mkΨ {
+  CΞ : symbols ;
+  Cξ : commlib ;
+  CKs : active_ectx ;
+}.
+#[local]
+Instance etaCfState : Settable _ := settable! mkΨ <CΞ; Cξ; CKs>.
+Record MemState : Type := mkΦ {
+  MH__ctx : heap ;
+  MH__comp : heap ;
+  MΔ : ptrstore ;
+}.
+#[local]
+Instance etaMemState : Settable _ := settable! mkΦ <MH__ctx; MH__comp; MΔ>.
+Record state : Type := mkΩ {
+  SF : CSC.Fresh.fresh_state ;
+  SΨ : CfState ;
+  St : ControlTag ;
+  SΦ : MemState ;
+}.
+#[local]
+Instance etaState : Settable _ := settable! mkΩ <SF; SΨ; St; SΦ>.
+
+Import RecordSetNotations.
+
+Definition Htgrow (Φ : MemState) (s : nat) (t : ControlTag) : option MemState :=
+  match t with
+  | CCtx => let* H := Hgrow Φ.(MH__ctx) s in Some(Φ <| MH__ctx := H |>)
+  | CComp => let* H := Hgrow Φ.(MH__comp) s in Some(Φ <| MH__comp := H |>)
+  end
+.
+Definition getH (Φ : MemState) (t : ControlTag) : heap :=
+  match t with
+  | CCtx => Φ.(MH__ctx)
+  | CComp => Φ.(MH__comp)
+  end
+.
+Definition setH (Φ : MemState) (t : ControlTag) (H : heap) : MemState :=
+  match t with
+  | CCtx => Φ <| MH__ctx := H |>
+  | CComp => Φ <| MH__comp := H |>
+  end
+.
+
+Notation "'Ψ(' Ξ ';' ξ ';' Ks ')'" := ({| CΞ := Ξ ; Cξ := ξ ; CKs := Ks |}) (at level 81, ξ at next level, Ks at next level).
+Notation "'Φ(' H__ctx ';' H__comp ';' Δ ')'" := ({| MH__ctx := H__ctx ; MH__comp := H__comp ; MΔ := Δ |}) (at level 81, H__comp at next level, Δ at next level).
+Notation "'Ωa(' F ';' Ψ ';' t ';' Φ ')'" := ({| SF := F ; SΨ := Ψ ; St := t ; SΦ := Φ |}) (at level 81, Ψ at next level, t at next level, Φ at next level).
+Notation "'Ω(' F ';' Ξ ';' ξ ';' Ks ';' t ';' H__ctx ';' H__comp ';' Δ ')'" :=
+  (Ωa(F ; (Ψ(Ξ ; ξ ; Ks) : CfState) ; t ; (Φ(H__ctx ; H__comp ; Δ) : MemState))) (at level 81, Δ at next level).
+Definition nodupinv (Ω : state) : Prop :=
+  nodupinv (Ω.(SΨ).(CΞ)) /\ nodupinv (Ω.(SΦ).(MH__ctx)) /\ nodupinv (Ω.(SΦ).(MH__comp)) /\ nodupinv (Ω.(SΦ).(MΔ))
+.
+Lemma nodupinv_empty (Ξ : symbols) (ξ : commlib) :
+  Util.nodupinv Ξ ->
+  nodupinv (Ω(Fresh.empty_fresh; Ξ; ξ; List.nil; CComp; hNil; hNil; snil)).
+Proof. intros H; cbn; repeat split; eauto; constructor. Qed.
+Lemma nodupinv_grow_H__ctx F Ξ ξ Ks t H__ctx H__comp Δ n H__ctx':
+  nodupinv (Ω(F;Ξ;ξ;Ks;t;H__ctx;H__comp;Δ)) ->
+  Hgrow H__ctx n = Some H__ctx' ->
+  nodupinv (Ω(F;Ξ;ξ;Ks;t;H__ctx';H__comp;Δ))
+.
+Proof.
+  intros [Ha [Hb [Hc Hd]]]; repeat split; eauto; cbn in Ha, Hb, Hc, Hd.
+  revert H__ctx' H__ctx Hb H; induction n; intros H' H Hb H0.
+  - now inv H0.
+  - cbn in H0. destruct (option_dec (Hgrow_aux H n (List.length (dom H)))) as [Hx|Hy]; try (rewrite Hy in H0; congruence).
+    apply not_eq_None_Some in Hx as [H__x Hx].
+    rewrite Hx in H0.
+    cbn in H0. now apply push_ok in H0.
+Qed.
+Lemma nodupinv_grow_H__comp F Ξ ξ Ks t H__ctx H__comp Δ n H__comp':
+  nodupinv (Ω(F;Ξ;ξ;Ks;t;H__ctx;H__comp;Δ)) ->
+  Hgrow H__comp n = Some H__comp' ->
+  nodupinv (Ω(F;Ξ;ξ;Ks;t;H__ctx;H__comp';Δ))
+.
+Proof.
+  intros [Ha [Hb [Hc Hd]]]; repeat split; eauto; cbn in Ha, Hb, Hc, Hd.
+  revert H__comp' H__comp Hc H; induction n; intros H' H Hc H0.
+  - now inv H0.
+  - cbn in H0. destruct (option_dec (Hgrow_aux H n (List.length (dom H)))) as [Hx|Hy]; try (rewrite Hy in H0; congruence).
+    apply not_eq_None_Some in Hx as [H__x Hx].
+    rewrite Hx in H0.
+    cbn in H0. now apply push_ok in H0.
+Qed.
+(** Types of events that may occur in a trace. *)
+Variant preevent : Type :=
+| Sstart : preevent
+| Send (v : value) : preevent
+| Salloc (ℓ : loc) (n : nat) : preevent
+| Sdealloc (ℓ : loc) : preevent
+| Sget (ℓ : loc) (n : nat) : preevent
+| Sset (ℓ : loc) (n : value) (v : value) : preevent
+| Scall (q : comms) (foo : vart) (arg : value) : preevent
+| Sret (q : comms) (v : value) : preevent
+.
+Definition preevent_eqb (e1 e2 : preevent) : bool :=
+  match e1, e2 with
+  | Sstart, Sstart => true
+  | Send n1, Send n2 => n1 == n2
+  | Salloc ℓ0 n0, Salloc ℓ1 n1 => andb (ℓ0 == ℓ1) (Nat.eqb n0 n1)
+  | Sdealloc ℓ0, Sdealloc ℓ1 => ℓ0 == ℓ1
+  | Sget ℓ0 n0, Sget ℓ1 n1 => andb (ℓ0 == ℓ1) (Nat.eqb n0 n1)
+  | Sset ℓ0 n0 v0, Sset ℓ1 n1 v1 => andb (andb (ℓ0 == ℓ1) (n0 == n1))
+                                              (v0 == v1)
+  | Scall q1 foo v0, Scall q2 bar v1 => andb (andb (String.eqb foo bar) (v0 == v1)) (q1 == q2)
+  | Sret q1 v0, Sret q2 v1 => andb (v0 == v1) (q1 == q2)
+  | _, _ => false
+  end
+.
+Lemma preevent_eqb_eq e1 e2 :
+  preevent_eqb e1 e2 = true <-> e1 = e2.
+Proof.
+  destruct e1, e2; cbn; split; intros; try easy; eq_to_defeq value_eqb; eq_to_defeq loc_eqb; eq_to_defeq comms_eqb.
+  - now inv H.
+  - apply Nat.eqb_eq in H0; inv H0. reflexivity.
+  - inv H; split; try easy. apply Nat.eqb_refl.
+  - now inv H.
+  - apply Nat.eqb_eq in H0; inv H0; reflexivity.
+  - inv H; split; try easy. apply Nat.eqb_refl.
+  - inv H; repeat split; easy.
+  - apply String.eqb_eq in H; inv H; reflexivity.
+  - inv H; repeat split; easy.
+  - inv H; split; easy.
+Qed.
+#[local]
+Instance preeventeq__Instance : HasEquality preevent := {
+  eq := preevent_eqb ;
+  eqb_eq := preevent_eqb_eq ;
+}.
+Variant event : Type :=
+| SCrash : event
+| Sev (e__b : preevent) (t : ControlTag) : event
+.
+Definition event_eqb (e1 e2 : event) : bool :=
+  match e1, e2 with
+  | SCrash, SCrash => true
+  | Sev e1 t1, Sev e2 t2 => andb (e1 == e2) (t1 == t2)
+  | _, _ => false
+  end
+.
+Lemma event_eqb_eq (e1 e2 : event) :
+  event_eqb e1 e2 = true <-> e1 = e2.
+Proof.
+  destruct e1, e2; cbn; split; intros; try easy; eq_to_defeq event_eqb.
+  eq_to_defeq preevent_eqb; eq_to_defeq control_tag_eq.
+  inv H; eq_to_defeq preevent_eqb; eq_to_defeq control_tag_eq.
+Qed.
+#[local]
+Instance eventeq__Instance : HasEquality event := {
+  eq := event_eqb ;
+  eqb_eq := event_eqb_eq ;
+}.
+Notation "'ev(' e ';' t ')'" := (Sev e t) (at level 81, t at next level).
+(** Pretty-printing function for better debuggability *)
+Definition string_of_preevent (e : preevent) :=
+  match e with
+  | (Sstart) => "Start"%string
+  | (Send v) => String.append ("End "%string) ("v"%string)
+  | (Salloc (addr ℓ) n) => String.append
+                      (String.append ("Alloc ℓ"%string) (string_of_nat ℓ))
+                      (String.append (" "%string) (string_of_nat n))
+  | (Sdealloc (addr ℓ)) => String.append ("Dealloc ℓ"%string) (string_of_nat ℓ)
+  | (Sget (addr ℓ) n) => String.append
+                    (String.append ("Get ℓ"%string) (string_of_nat ℓ))
+                    (String.append (" "%string) (string_of_nat n))
+  | (Sset (addr ℓ) n m) => String.append
+                             (String.append
+                               (String.append ("Set ℓ"%string) (string_of_nat ℓ))
+                               (String.append (" "%string) ("n"%string)))
+                             (String.append (" "%string) ("m"%string))
+  | (Scall q foo v) => String.append (String.append
+                                     (String.append ("Call "%string)
+                                      (String.append (string_of_comms q)
+                                       (String.append " "%string foo))) " "%string)
+                      ("v"%string)
+  | (Sret q v) => String.append ("Ret "%string)
+                 (String.append (string_of_comms q)
+                  (String.append " "%string "v"%string))
+  end
+.
+Definition string_of_event (e : event) :=
+  match e with
+  | SCrash => "↯"%string
+  | Sev e__b t => String.append (string_of_preevent e__b) (string_of_controltag t)
+  end
+.
+
+(** A runtime program is a state plus an expression. *)
+Inductive rtexpr : Type :=
+| RTerm (Ω : state) (e : expr)
+| RCrash
+.
+(* '▷' is `\triangleright and '↯' is `\lightning`` *)
+Notation "Ω '▷' e" := ((RTerm Ω e) : rtexpr) (at level 81, e at next level).
+Notation "'↯' '▷' 'stuck'" := (RCrash).
+
+(** Substitution, which assumes that the given expression is closed. *)
+Definition subst (what : vart) (inn forr : expr) : expr :=
+  let fix R e :=
+    match e with
+    | Xval _ => e
+    | Xabort => Xabort
+    | Xlet x e0 e1 => if vareq what x then Xlet x (R e0) e1 else Xlet x (R e0) (R e1)
+    | Xnew e => Xnew (R e)
+    | Xdel e => Xdel (R e)
+    | Xget e0 e1 e2 => Xget (R e0) (R e1) (R e2)
+    | Xset e0 e1 e2 e3 => Xset (R e0) (R e1) (R e2) (R e3)
+    | Xvar x => if vareq what x then forr else e
+    | Xbinop b e1 e2 => Xbinop b (R e1) (R e2)
+    | Xifz c e1 e2 => Xifz (R c) (R e1) (R e2)
+    | Xreturn e => Xreturn (R e)
+    | Xcall foo e => Xcall foo (R e)
+    | Xunpack γ x e0 e1 => if vareq what x then Xunpack γ x (R e0) e1 else Xunpack γ x (R e0) (R e1)
+    | Xpack ℓ e => Xpack ℓ (R e)
+    | Xpair e0 e1 => Xpair (R e0) (R e1)
+    | Xunpair x1 x2 e0 e1 => if orb (vareq what x1) (vareq what x2) then
+                              Xunpair x1 x2 (R e0) e1
+                            else
+                              Xunpair x1 x2 (R e0) (R e1)
+    end
+  in
+  R inn
+.
+Inductive pstep : PrimStep rtexpr event :=
+| e_binop : forall (Ω : state) (n1 n2 n3 : nat) (b : binopsymb),
+    Some(Vnat n3) = eval_binop b n1 n2 ->
+    Ω ▷ Xbinop b (Xval n1) (Xval n2) --[]--> Ω ▷ (Xval n3)
+| e_ifz_true : forall (Ω : state) (e1 e2 : expr),
+    Ω ▷ Xifz (Xval 0) e1 e2 --[]--> Ω ▷ e1
+| e_ifz_false : forall (Ω : state) (e1 e2 : expr) (n : nat),
+    n <> 0 ->
+    Ω ▷ Xifz (Xval n) e1 e2 --[]--> Ω ▷ e2
+| e_abort : forall (Ω : state),
+    Ω ▷ Xabort --[ (SCrash) ]--> ↯ ▷ stuck
+| e_let : forall (Ω : state) (x : vart) (v : value) (e e' : expr),
+    e' = subst x e (Xval v) ->
+    Ω ▷ Xlet x (Xval v) e --[]--> Ω ▷ e'
+| e_unpair : forall (Ω : state) (v1 v2 : value) (x1 x2 : vart) (e e' : expr),
+    e' = subst x1 (subst x2 e (Xval v2)) (Xval v1) ->
+    Ω ▷ Xunpair x1 x2 (Xval(Vpair v1 v2)) e --[]--> Ω ▷ e'
+| e_alloc : forall (F F' : CSC.Fresh.fresh_state) (Ψ : CfState) (t : ControlTag)
+              (Φ Φ' : MemState) (n : nat) (ℓ : loc) (Δ' : ptrstore),
+    ℓ = addr(Fresh.fresh F) ->
+    F' = Fresh.advance F ->
+    push ℓ (dL(ℓ ; ◻ ; t ; n)) Φ.(MΔ) = Some Δ' ->
+    Some Φ' = Htgrow (Φ <| MΔ := Δ' |>) n t ->
+    (Ωa(F ; Ψ ; t ; Φ)) ▷ Xnew (Xval n) --[ ev( Salloc ℓ n ; t ) ]--> (Ωa(F' ; Ψ ; t ; Φ)) ▷ (Xval (Vpack (LConst ℓ) (Vpair Vcap (Vptr ℓ))))
+| e_delete : forall (F : CSC.Fresh.fresh_state) (Ψ : CfState) (t : ControlTag)
+               (Φ Φ' : MemState) (n : nat) (ℓ : loc) (ρ : poison) (Δ1 Δ2 : ptrstore),
+    Util.nodupinv (Δ1 ◘ ℓ ↦ (dL(ℓ ; ρ ; t ; n)) ◘ Δ2) ->
+    Φ' = Φ <| MΔ := Δ1 ◘ ℓ ↦ (dL(ℓ ; ☣ ; t ; n)) ◘ Δ2 |> ->
+    Ωa(F ; Ψ ; t ; Φ) ▷ Xdel (Xval (Vpack (LConst ℓ) (Vpair Vcap (Vptr ℓ)))) --[ ev( Sdealloc ℓ ; t ) ]--> Ωa(F ; Ψ ; t ; Φ') ▷ Xval 0
+| e_get : forall (F : CSC.Fresh.fresh_state) (Ψ : CfState) (t : ControlTag)
+            (Φ : MemState) (n m ℓ : nat) (v : value)  (ρ : poison) (Δ1 Δ2 : ptrstore),
+    Util.nodupinv (Δ1 ◘ (addr ℓ) ↦ dL(addr ℓ ; ρ ; t ; n) ◘ Δ2) ->
+    (mget (getH Φ t) (ℓ + n) = Some(Some v) \/ v = Vnat 1729) ->
+    Ωa(F ; Ψ ; t ; Φ) ▷ Xget (Xval Vcap) (Xval(Vptr (addr ℓ))) (Xval n) --[ ev( Sget (addr ℓ) n ; t ) ]--> Ωa(F ; Ψ ; t ; Φ) ▷ Xval v
+| e_set : forall (F : CSC.Fresh.fresh_state) (Ψ : CfState) (t : ControlTag) (H' : heap)
+            (Φ Φ' : MemState) (n m ℓ v : nat) (w : value) (ρ : poison) (Δ1 Δ2 : ptrstore),
+    Util.nodupinv (Δ1 ◘ (addr ℓ) ↦ dL(addr ℓ ; ρ ; t ; n) ◘ Δ2) ->
+    (mset (getH Φ t) (ℓ + n) (Some w) = Some H' \/ H' = getH Φ t) ->
+    Φ' = setH Φ t H' ->
+    Ωa(F ; Ψ ; t ; Φ) ▷ Xset (Xval Vcap) (Xval(Vptr (addr ℓ))) (Xval n) (Xval w) --[ ev( Sset (addr ℓ) n w ; t ) ]--> Ωa(F ; Ψ ; t ; Φ') ▷ Xval w
+| e_unpack : forall (Ω : state) (γ x : vart) (ℓ : loc) (v : value) (e e' : expr),
+    e' = subst γ (subst x e (Xval v)) (Xval (Vptr ℓ)) ->
+    Ω ▷ Xunpack γ x (Xval (Vpack (LConst ℓ) v)) e --[]--> Ω ▷ e'
+.
+#[global]
+Existing Instance pstep.
+#[global]
+Hint Constructors pstep : core.
+
+Lemma pstep_is_nodupinv_invariant Ω e Ω' e' a :
+  Ω ▷ e --[, a ]--> Ω' ▷ e' ->
+  nodupinv Ω ->
+  nodupinv Ω'
+.
+Proof.
+  remember (Ω ▷ e) as r0; remember (Ω' ▷ e') as r1.
+  induction 1; inv Heqr0; inv Heqr1; try easy.
+  - (* e_delete *) admit.
+  - (* e_set *) admit.
+Admitted.
+
+(** functional version of the above *)
+Definition pstepf (r : rtexpr) : option (option event * rtexpr) :=
+  None (* TODO *)
+.
+Ltac grab_value e :=
+  (destruct e as [[[[e]|]|]| | | | | | | | | |]; try congruence)
+.
+Ltac grab_value2 e1 e2 := (grab_value e1; grab_value e2).
+
+Lemma Hget_none (H : heap) (n : nat) :
+  n >= length H -> mget H n = None.
+Proof. Admitted.
+Lemma Hget_some (H : heap) (n : nat) :
+  n < length H -> exists v, mget H n = Some v.
+Proof. Admitted.
+Lemma Hset_none (H : heap) (n : nat) v :
+  n >= length H -> mset H n v = None.
+Proof. Admitted.
+Lemma Hset_some (H : heap) (n : nat) v :
+  n < length H -> exists H', mset H n v = Some H'.
+Proof. Admitted.
+
+(** We use an alternative notation of pstep here that does not constrain a to be *either* Some/None *)
+Lemma equiv_pstep (r0 : rtexpr) (a : option event) (r1 : rtexpr) :
+  r0 --[, a ]--> r1 <-> pstepf r0 = Some(a, r1).
+Proof.
+Admitted.
+Lemma pstepf_is_nodupinv_invariant Ω e Ω' e' a :
+  pstepf (Ω ▷ e) = Some(a, Ω' ▷ e') ->
+  nodupinv Ω ->
+  nodupinv Ω'
+.
+Proof. intros H0 H1; apply equiv_pstep in H0; apply pstep_is_nodupinv_invariant in H0; eauto. Qed.
+
+(** convert an expression to evalctx in order to execute it functionally + "contextually" *)
+(** this function returns an eval context K and an expr e' such that K[e'] = e given some e *)
+Fixpoint evalctx_of_expr (e : expr) : option (evalctx * expr) :=
+  match e with
+  | Xval _ => None
+  | Xvar _ => None
+  | Xdel x => Some(Khole, Xdel x)
+  | Xabort => Some(Khole, Xabort)
+  | Xbinop b e1 e2 =>
+    match e1, e2 with
+    | Xres(Fres(Fval(Vnat n1))), Xres(Fres(Fval(Vnat n2))) =>
+      Some(Khole, Xbinop b n1 n2)
+    | Xres(Fres(Fval(Vnat n1))), en2 =>
+      let* (K, e2') := evalctx_of_expr en2 in
+      Some(KbinopR b n1 K, e2')
+    | _, _ =>
+      let* (K, e1') := evalctx_of_expr e1 in
+      Some(KbinopL b K e2, e1')
+    end
+  | Xget x en =>
+    match en with
+    | Xres(Fres(Fval(Vnat n))) =>
+      Some(Khole, Xget x n)
+    | _ => let* (K, en') := evalctx_of_expr en in
+          Some(Kget x K, en')
+    end
+  | Xset x en ev =>
+    match en, ev with
+    | Xres(Fres(Fval(Vnat n))), Xres(Fres(Fval(Vnat v))) =>
+      Some (Khole, Xset x n v)
+    | Xres(Fres(Fval(Vnat n))), ev =>
+      let* (K, ev') := evalctx_of_expr ev in
+      Some(KsetR x n K, ev')
+    | en, ev =>
+      let* (K, en') := evalctx_of_expr en in
+      Some(KsetL x K ev, en')
+    end
+  | Xlet x e1 e2 =>
+    match e1 with
+    | Xres(Fres f) =>
+      Some(Khole, Xlet x f e2)
+    | _ => let* (K, e1') := evalctx_of_expr e1 in
+          Some(Klet x K e2, e1')
+    end
+  | Xnew x e1 e2 =>
+    match e1 with
+    | Xres(Fres(Fval(Vnat n))) =>
+      Some(Khole, Xnew x n e2)
+    | _ => let* (K, e1') := evalctx_of_expr e1 in
+          Some(Knew x K e2, e1')
+    end
+  | Xreturn e =>
+    match e with
+    | Xres f =>
+      Some(Khole, Xreturn f)
+    | _ => let* (K, e') := evalctx_of_expr e in
+          Some(Kreturn K, e')
+    end
+  | Xcall foo e =>
+    match e with
+    | Xres f =>
+      Some(Khole, Xcall foo f)
+    | _ => let* (K, e') := evalctx_of_expr e in
+          Some(Kcall foo K, e')
+    end
+  | Xifz c e0 e1 =>
+    match c with
+    | Xres(Fres(Fval(Vnat v))) =>
+      Some(Khole, Xifz v e0 e1)
+    | _ => let* (K, c') := evalctx_of_expr c in
+          Some(Kifz K e0 e1, c')
+    end
+  end
+.
+(* Checks wether the thing that is filled into the hole is somehow structurually compatible with pstep *)
+Definition pstep_compatible (e : expr) : option expr :=
+  match e with
+  | Xifz 0 e0 e1 => Some (Xifz 0 e0 e1)
+  | Xifz (S n) e0 e1 => Some (Xifz (S n) e0 e1)
+  | Xabort => Some (Xabort)
+  | Xdel x => Some (Xdel x)
+  | Xbinop b (Xres(Fres(Fval(Vnat n1)))) (Xres(Fres(Fval(Vnat n2)))) => Some (Xbinop b n1 n2)
+  | Xget x (Xres(Fres(Fval(Vnat n)))) => Some(Xget x n)
+  | Xset x (Xres(Fres(Fval(Vnat n1)))) (Xres(Fres(Fval(Vnat n2)))) => Some(Xset x n1 n2)
+  | Xnew x (Xres(Fres(Fval(Vnat n)))) e => Some(Xnew x n e)
+  | Xlet x (Xres(Fres f)) e => Some(Xlet x f e)
+  | _ => None
+  end
+.
+Definition pestep_compatible (e : expr) : option expr :=
+  match e with
+  | Xifz 0 e0 e1 => Some (Xifz 0 e0 e1)
+  | Xifz (S n) e0 e1 => Some (Xifz (S n) e0 e1)
+  | Xabort => Some (Xabort)
+  | Xdel x => Some (Xdel x)
+  | Xbinop b (Xres(Fres(Fval(Vnat n1)))) (Xres(Fres(Fval(Vnat n2)))) => Some (Xbinop b n1 n2)
+  | Xget x (Xres(Fres(Fval(Vnat n)))) => Some(Xget x n)
+  | Xset x (Xres(Fres(Fval(Vnat n1)))) (Xres(Fres(Fval(Vnat n2)))) => Some(Xset x n1 n2)
+  | Xnew x (Xres(Fres(Fval(Vnat n)))) e => Some(Xnew x n e)
+  | Xlet x (Xres(Fres f)) e => Some(Xlet x f e)
+  | Xcall foo (Xres(Fres f)) => Some(Xcall foo f)
+  | Xreturn (Xres(Fres f)) => Some(Xreturn f)
+  | _ => None
+  end
+.
+Lemma return_pestep_compat (f : fnoerr) :
+  Some(Xreturn f) = pestep_compatible (Xreturn f).
+Proof. now cbn. Qed.
+Lemma call_pestep_compat foo (f : fnoerr) :
+  Some(Xcall foo f) = pestep_compatible (Xcall foo f).
+Proof. now cbn. Qed.
+Lemma pstep_compat_weaken e :
+  Some e = pstep_compatible e ->
+  Some e = pestep_compatible e.
+Proof. induction e; now cbn. Qed.
+#[global]
+Hint Resolve pstep_compat_weaken call_pestep_compat return_pestep_compat : core.
+
+(** ** Environment Semantics extended with context switches *)
+(** ρ__call judgement takes care of emitting Qinternal or Qctxtocomp/Qcomptoctx, depending on whether
+    the current context and the new context is in the list of components ξ or not. *)
+Inductive ρ__call : commlib -> vart -> vart -> fnoerr -> option event -> comms -> Prop :=
+| comm_call_comptoctx : forall ξ foo bar iv,
+    ~(List.In foo ξ) ->
+    List.In bar ξ ->
+    ρ__call ξ foo bar iv (Some(Scall Qcomptoctx foo iv)) Qctxtocomp
+| comm_call_ctxtocomp : forall ξ foo bar iv,
+    List.In foo ξ ->
+    ~(List.In bar ξ) ->
+    ρ__call ξ foo bar iv (Some(Scall Qctxtocomp foo iv)) Qcomptoctx
+| comm_call_internal_comp : forall ξ foo bar iv,
+    List.In foo ξ ->
+    List.In bar ξ ->
+    ρ__call ξ foo bar iv None Qinternal
+| comm_call_internal_ctx : forall ξ foo bar iv,
+    ~(List.In foo ξ) ->
+    ~(List.In bar ξ) ->
+    ρ__call ξ foo bar iv None Qinternal
+.
+Definition ρf__call (ξ : commlib) (new cur : vart) (f : fnoerr) : (option event) * comms :=
+  match List.find (fun x => vareq x new) ξ, List.find (fun x => vareq x cur) ξ with
+  | None, None | Some _, Some _ => (None, Qinternal)
+  | None, Some _ => (* we call from component into context, so this is Qcomptoctx *)
+    (Some(Scall Qcomptoctx new f), Qctxtocomp)
+  | Some _, None => (* we call from context into component, so this is Qctxtocomp *)
+    (Some(Scall Qctxtocomp new f), Qcomptoctx)
+  end
+.
+Ltac In_find_resolve_contr_hook Hx Hy := fail.
+Ltac In_find_resolve_contr := (
+      match goal with
+      | [Hx : List.find (fun x : string => vareq _ ?bar) ?ξ = None,
+         Hy : In ?bar ?ξ |- _] =>
+        apply (List.find_none _ _ Hx) in Hy; apply String.eqb_neq in Hy; contradiction
+      | [Hx : List.find (fun x : string => vareq _ ?bar) ?ξ = Some _,
+         Hy : ~In ?bar ?ξ |- _] =>
+        let Hxf := fresh "Hx'" in
+        let Hx1 := fresh "Hx1" in
+        let Hx2 := fresh "Hx2" in
+        assert (Hx':=Hx); apply List.find_some in Hxf as [Hx1 Hx2];
+        apply String.eqb_eq in Hx2; subst; contradiction
+      | [Hx : List.find (fun x : string => vareq _ ?foo) _ = None,
+         Hy : List.find (fun x : string => vareq _ ?bar) _ = None |- _] =>
+        In_find_resolve_contr_hook Hx Hy
+      | [Hx : List.find (fun x : string => vareq _ ?foo) _ = Some _,
+         Hy : List.find (fun x : string => vareq _ ?bar) _ = Some _ |- _] =>
+        In_find_resolve_contr_hook Hx Hy
+      end)
+.
+Lemma dup (A : Prop) : A -> A /\ A.
+Proof. now split. Qed.
+Ltac option_boilerplate H := (
+    let Hx := fresh "Hx" in
+    let Hx' := fresh "Hx" in
+    let x := fresh "x" in
+    destruct (option_dec H) as [Hx | Hx]; try
+    (apply not_eq_None_Some in Hx as [x Hx']; apply dup in Hx' as [Hx Hx'])
+    )
+.
+Lemma ρ__call_equiv_ρf__call (ξ : commlib) (new cur : vart) (f : fnoerr) (a : option event) (q : comms) :
+  ρ__call ξ new cur f a q <-> ρf__call ξ new cur f = (a, q)
+.
+Proof.
+  split.
+  - Ltac In_find_resolve_contr_hook Hx Hy ::= now (unfold ρf__call; rewrite Hx, Hy).
+    option_boilerplate (List.find (fun x => vareq x new) ξ); option_boilerplate (List.find (fun x => vareq x cur) ξ);
+    destruct 1; try In_find_resolve_contr; try now unfold ρf__call; rewrite Hx, Hx1.
+  - option_boilerplate (List.find (fun x => vareq x new) ξ); option_boilerplate (List.find (fun x => vareq x cur) ξ);
+    unfold ρf__call; intros H.
+    + rewrite Hx, Hx1 in H; inv H. apply List.find_some in Hx as [Hy1 Hy2], Hx1 as [Hy3 Hy4].
+      apply String.eqb_eq in Hy2, Hy4; subst.
+      now constructor.
+    + rewrite Hx, Hx1 in H; inv H. eapply List.find_some in Hx as [Hy1 Hy2].
+      eapply String.eqb_eq in Hy2; subst.
+      constructor; eauto. intros H.
+      apply (List.find_none _ _ Hx1) in H. apply String.eqb_neq in H; contradiction.
+    + rewrite Hx, Hx0 in H; inv H. apply List.find_some in Hx0 as [Hy1 Hy2].
+      eapply String.eqb_eq in Hy2; subst.
+      constructor; eauto; intros H.
+      apply (List.find_none _ _ Hx) in H. apply String.eqb_neq in H; contradiction.
+    + rewrite Hx, Hx0 in H; inv H.
+      constructor 4; intros H.
+      apply (List.find_none _ _ Hx) in H; apply String.eqb_neq in H; contradiction.
+      apply (List.find_none _ _ Hx0) in H; apply String.eqb_neq in H; contradiction.
+Qed.
+
+Inductive ρ__ret : comms -> fnoerr -> option event -> Prop :=
+| comm_ret_ctxtocomp : forall f,
+    ρ__ret Qctxtocomp f (Some(Sret Qctxtocomp f))
+| comm_ret_comptoctx : forall f,
+    ρ__ret Qcomptoctx f (Some(Sret Qcomptoctx f))
+| comm_ret_internal : forall f,
+    ρ__ret Qinternal f None
+.
+Definition ρf__ret (a : comms) (b : fnoerr) : option event :=
+  match a with
+  | Qctxtocomp | Qcomptoctx => Some(Sret a b)
+  | _ => None
+  end
+.
+Lemma ρ__ret_equiv_ρf__ret (a : comms) (b : fnoerr) (c : option event) :
+  ρ__ret a b c <-> ρf__ret a b = c
+.
+Proof.
+  split.
+  - now destruct 1.
+  - destruct a; cbn; inversion 1; auto using comm_ret_ctxtocomp, comm_ret_comptoctx, comm_ret_internal.
+Qed.
+Inductive estep : CtxStep :=
+| E_ctx : forall (Ω Ω' : state) (e e' e0 e0' : expr) (a : option event) (K : evalctx),
+    (*Some(K,e) = evalctx_of_expr e0 ->*)
+    Some e = pstep_compatible e ->
+    e0 = insert K e ->
+    e0' = insert K e' ->
+    Ω ▷ e --[, a ]--> Ω' ▷ e' ->
+    Ω ▷ e0 ==[, a ]==> Ω' ▷ e0'
+| E_abrt_ctx : forall (Ω : state) (e e0 : expr) (K : evalctx),
+    (*Some(K,e) = evalctx_of_expr e0 ->*)
+    Some e = pstep_compatible e ->
+    e0 = insert K e ->
+    Ω ▷ e --[ Scrash ]--> ↯ ▷ stuck ->
+    Ω ▷ e0 ==[ Scrash ]==> ↯ ▷ stuck
+| E_call_main : forall (F : CSC.Fresh.fresh_state) (Ξ : symbols) (ξ : commlib) (H : heap) (Δ : store)
+                  (e__foo : expr) (x__arg : vart),
+    Some (x__arg, (Tectx(Tarrow Tℕ Tℕ)), e__foo) = mget Ξ "main"%string ->
+    (F ; Ξ ; ξ ; List.nil ; H ; Δ ▷ insert Khole (Xcall "main"%string 0) ==[ Sstart ]==> F ; Ξ ; ξ ; (Khole, "main"%string, Qctxtocomp) :: List.nil ; H ; Δ ▷ Xreturn (subst x__arg e__foo 0))
+| E_call : forall (F : CSC.Fresh.fresh_state) (Ξ : symbols) (ξ : commlib) (K : active_ectx) (H : heap) (Δ : store)
+             (E E__K : evalctx) (e__foo : expr) (τ__foo : Ty) f (x__arg foo foo__K : vart) (q q__K : comms) (a : option event),
+    Some (x__arg, τ__foo, e__foo) = mget Ξ foo ->
+    ρ__call ξ foo foo__K f a q ->
+    (F ; Ξ ; ξ ; (E__K, foo__K, q__K) :: K ; H ; Δ ▷ insert E (Xcall foo f) ==[, a ]==> F ; Ξ ; ξ ; (E, foo, q) :: (E__K, foo__K, q__K) :: K ; H ; Δ ▷ Xreturn (subst x__arg e__foo f))
+| E_ret : forall (F : CSC.Fresh.fresh_state) (Ξ : symbols) (ξ : commlib) (K : active_ectx) (H : heap) (Δ : store)
+            (E E' : evalctx) (foo : vart) (q : comms) f (a : option event),
+    ρ__ret q f a ->
+    K <> List.nil ->
+    (F ; Ξ ; ξ ; (E, foo, q) :: K ; H ; Δ ▷ insert E' (Xreturn f) ==[, a ]==> F ; Ξ ; ξ ; K ; H ; Δ ▷ insert E f)
+| E_ret_end : forall (F : CSC.Fresh.fresh_state) (Ξ : symbols) (ξ : commlib) (K : active_ectx) (H : heap) (Δ : store) f (E : evalctx),
+    (F ; Ξ ; ξ ; (Khole, "main"%string, Qcomptoctx) :: List.nil ; H ; Δ ▷ insert E (Xreturn (Fval f)) ==[ Send f ]==> F ; Ξ ; ξ ; List.nil ; H ; Δ ▷ f)
+.
+#[global]
+Existing Instance estep.
+#[global]
+Hint Constructors estep : core.
+
+Lemma estep_is_nodupinv_invariant Ω e Ω' e' a :
+  Ω ▷ e ==[, a ]==> Ω' ▷ e' ->
+  nodupinv Ω ->
+  nodupinv Ω'
+.
+Proof.
+  assert (Some Ω = let (oΩ, e) := Ω ▷ e in oΩ) by easy;
+  assert (Some Ω' = let (oΩ', e') := Ω' ▷ e' in oΩ') by easy;
+  induction 1; try (inv H; inv H0; easy);
+  inv H; inv H0; intros H0; apply pstep_is_nodupinv_invariant in H4; eauto.
+Qed.
+Local Set Warnings "-cast-in-pattern".
+Ltac crush_estep := (match goal with
+                     | [H: _ ▷ (Xres ?f) ==[ ?a ]==> ?r |- _] =>
+                       inv H
+                     | [H: _ ▷ (Xres ?f) ==[]==> ?r |- _] =>
+                       inv H
+                     | [H: _ ▷ (Xres ?f) ==[, ?a ]==> ?r |- _] =>
+                       inv H
+                     end);
+  (repeat match goal with
+   | [H: insert ?E (Xreturn (Xres(Fres ?f0))) = Xres ?f |- _] => induction E; try congruence; inv H
+   | [H: insert ?E (Xcall ?foo (Xres(Fres ?f0))) = Xres ?f |- _] => induction E; try congruence; inv H
+   | [H: Xres ?f = insert ?K ?e |- _] =>
+     induction K; cbn in H; try congruence; inv H
+   | [H: _ ▷ (Xres ?f) --[]--> ?r |- _] =>
+     inv H
+   | [H: _ ▷ (Xres ?f) --[, ?a ]--> ?r |- _] =>
+     inv H
+   | [H: _ ▷ (Xres ?f) --[ ?a ]--> ?r |- _] =>
+     inv H
+   end)
+.
+Ltac unfold_estep := (match goal with
+                      | [H: _ ▷ _ ==[ _ ]==> _ ▷ _ |- _ ] => inv H
+                      end);
+  (match goal with
+   | [H: _ = insert ?K _ |- _] =>
+     induction K; cbn in H; try congruence; inv H
+   end).
+
+Definition estepf (r : rtexpr) : option (option event * rtexpr) :=
+  let '(oΩ, e) := r in
+  let* Ω := oΩ in
+  let* (K, e0) := evalctx_of_expr e in
+  match e0 with
+  | Xcall foo (Xres(Fres f)) =>
+    let '(F, Ξ, ξ, Ks', H, Δ) := Ω in
+    match mget Ξ foo with
+    | None => None
+    | Some (argx, τ__arg, e__foo) =>
+      match Ks' with
+      | List.nil =>
+        if vareq foo "main"%string then
+          Some(Some Sstart, (F ; Ξ ; ξ ; (Khole, "main"%string, Qctxtocomp) :: List.nil ; H ; Δ ▷ (Xreturn (subst argx e__foo 0))))
+        else
+          None
+      | (K__bar, bar, q) :: Ks =>
+        match ρf__call ξ foo bar f with
+        | (a, q') =>
+          Some(a, (F ; Ξ ; ξ ; ((K, foo, q') :: (K__bar, bar, q) :: Ks) ; H ; Δ ▷ (Xreturn (subst argx e__foo f))))
+        end
+      end
+    end
+  | Xreturn(Xres(Fres f)) =>
+    let '(F, Ξ, ξ, Ks', H, Δ) := Ω in
+    match Ks' with
+    | nil => None
+    | (Khole, "main"%string, Qctxtocomp) :: List.nil =>
+      match f with
+      | Fval(v) => Some(Some(Send v), F ; Ξ ; ξ ; List.nil ; H ; Δ ▷ f)
+      | _ => None
+      end
+    | (K__foo, _foo, q) :: Ks =>
+      let a := ρf__ret q f in
+      Some(a, F ; Ξ ; ξ ; Ks ; H ; Δ ▷ insert K__foo f)
+    end
+  | _ =>
+    let* _ := pstep_compatible e0 in
+    let* (a, (oΩ, e0')) := pstepf (Ω ▷ e0) in
+    match oΩ with
+    | None => Some(Some(Scrash), ↯ ▷ stuck)
+    | Some Ω' => Some(a, Ω' ▷ insert K e0')
+    end
+  end
+.
+
+Ltac crush_insert :=
+  match goal with
+  | [H: insert ?K ?e = ?f |- _] => symmetry in H
+  | _ => trivial
+  end;
+  (match goal with
+   | [H: ?f = insert ?K ?e |- _] =>
+     let H' := fresh "H" in
+     assert (H':=H); generalize dependent e; induction K; intros; cbn in H; try congruence; inv H
+   end)
+.
+
+Inductive is_val : expr -> Prop :=
+| Cfres : forall e f, e = Xres(Fres(Fval(Vnat f))) -> is_val e
+.
+
+Lemma expr_val_dec e :
+  { is_val e } + { ~is_val e }.
+Proof.
+  induction e.
+  1: destruct f. destruct f. destruct v. left; eauto using Cfres.
+  all: right; intros H; inv H; inv H0.
+Qed.
+#[local]
+Ltac crush_grab_ectx :=
+      (repeat match goal with
+      | [H: Some(Xres ?f) = pestep_compatible(Xres ?f) |- _] => inv H
+      | [H: Some(?e) = pestep_compatible ?e |- _] => cbn in H
+      | [H: Some(_) = match ?e with
+                      | Xres _ => _
+                      | _ => _
+                      end |- _] => grab_value e
+      | [H: Some _ = None |- _] => inv H
+      end; try now cbn;
+      match goal with
+      | [v : value |- _] => destruct v
+      | [ |- _ ] => trivial
+      end;
+      cbn; repeat match goal with
+           | [H1: _ = insert _ _ |- _] => cbn in H1
+           | [H: Some ?e0 = pestep_compatible ?e0 |- match insert ?K ?e0 with
+                                                   | Xres _ => _
+                                                   | _ => _
+                                                   end = _] => let ek := fresh "ek" in
+                                                              let H2 := fresh "H2" in
+                                                              remember (insert K e0) as ek;
+                                                              destruct (expr_val_dec ek) as [H2|H2];
+                                                              try (inv H2; crush_insert; match goal with
+                                                              | [H: Some ?f = pestep_compatible ?f, f: nat |- _] => inv H
+                                                              end)
+           | [H: Some(?e0) = pestep_compatible ?e0,
+             H1: _ = insert _ _ |- _] => cbn in H
+           end;
+      match goal with
+      | [K: evalctx, e0: expr, ek: expr,
+         H: Some ?e0 = pestep_compatible ?e0,
+         Heqek: ?ek = insert ?K ?e0,
+         IHe: (forall (K' : evalctx) (e0' : expr), Some e0' = pestep_compatible e0' ->
+                                              ?ek = insert K' e0' ->
+                                              evalctx_of_expr ?ek = Some(K', e0'))
+         |- _] =>
+         specialize (IHe K e0 H Heqek) as ->
+      end;
+      repeat match goal with
+      | [H: ~ is_val ?ek |- match ?ek with
+                           | Xres _ => _
+                           | _ => _
+                           end = _] => destruct ek; trivial
+      | [H: ~ is_val (Xres ?f) |- match ?f with
+                          | Fres _ => _
+                          | _ => _
+                          end = _] => destruct f; trivial
+      | [H: ~ is_val (Xres(Fres ?f)) |- match ?f with
+                          | Fval _ => _
+                          | _ => _
+                          end = _] => destruct f; trivial
+      | [H: ~ is_val (Xres(Fres(Fval ?v))) |- _ ] => destruct v; destruct H; eauto using Cfres
+      end).
+Lemma grab_ectx e K e0 :
+  Some e0 = pestep_compatible e0 ->
+  e = insert K e0 ->
+  evalctx_of_expr e = Some(K, e0)
+.
+Proof.
+  revert K e0; induction e; intros; crush_insert; crush_grab_ectx.
+  cbn. remember (insert K e0) as ek.
+  destruct (expr_val_dec ek) as [H2|H2];
+  try (inv H2; crush_insert; inv H).
+  specialize (IHe1 K e0 H Heqek) as ->.
+  destruct ek; trivial. destruct f; trivial.
+  induction K; cbn in Heqek; try congruence; inv Heqek; inv H.
+
+  cbn; remember (insert K e0) as ek.
+  destruct (expr_val_dec ek) as [H2|H2];
+  try (inv H2; crush_insert; inv H).
+  specialize (IHe K e0 H Heqek) as ->;
+  destruct ek; trivial.
+  induction K; cbn in Heqek; try congruence; inv Heqek; inv H.
+
+  cbn; remember (insert K e0) as ek.
+  destruct (expr_val_dec ek) as [H2|H2];
+  try (inv H2; crush_insert; inv H).
+  specialize (IHe K e0 H Heqek) as ->;
+  destruct ek; trivial.
+  induction K; cbn in Heqek; try congruence; inv Heqek; inv H.
+Qed.
+
+Lemma easy_ectx e0 :
+  Some e0 = pestep_compatible e0 ->
+  evalctx_of_expr e0 = Some(Khole, e0).
+Proof. induction e0; cbn in *; intros H; crush_grab_ectx. Qed.
+
+Lemma injective_ectx e0 K e e' :
+  Some e0 = pestep_compatible e0 ->
+  evalctx_of_expr e = Some(K, e0) ->
+  evalctx_of_expr e' = Some(K, e0) ->
+  e = e'.
+Proof. Admitted.
+
+Lemma ungrab_ectx e K e0 :
+  Some e0 = pestep_compatible e0 ->
+  evalctx_of_expr e = Some(K, e0) ->
+  e = insert K e0.
+Proof.
+  intros H H1; remember (insert K e0) as e1;
+  eapply grab_ectx in Heqe1 as H2; eauto;
+  eapply injective_ectx; eauto.
+Qed.
+Lemma pstep_compatible_some e e' :
+  pstep_compatible e = Some e' -> e = e'.
+Proof.
+  revert e'; induction e; intros; cbn in H; try congruence.
+  - (* binop *) grab_value2 e1 e2.
+  - (* get *) grab_value e.
+  - (* set *) grab_value2 e1 e2.
+  - (* let *) grab_value e1.
+  - (* new *) grab_value e1.
+  - (* ifz *) grab_value e1; destruct e1; now inv H.
+Qed.
+
+Lemma pestep_compatible_some e e' :
+  pestep_compatible e = Some e' -> e = e'.
+Proof.
+  revert e'; induction e; intros; cbn in H; try congruence.
+  - (* binop *) grab_value2 e1 e2.
+  - (* get *) grab_value e.
+  - (* set *) grab_value2 e1 e2.
+  - (* let *) grab_value e1.
+  - (* new *) grab_value e1.
+  - (* ret *) grab_value e.
+  - (* call *) grab_value e.
+  - (* ifz *) grab_value e1; destruct e1; now inv H.
+Qed.
+Lemma elim_ectx_ret K (f : fnoerr) :
+  evalctx_of_expr (insert K (Xreturn f)) = Some(K, Xreturn f).
+Proof. remember (insert K (Xreturn f)); eapply grab_ectx in Heqe; eauto. Qed.
+Lemma elim_ectx_call K foo (f : fnoerr) :
+  evalctx_of_expr (insert K (Xcall foo f)) = Some(K, Xcall foo f).
+Proof. remember (insert K (Xcall foo f)); eapply grab_ectx in Heqe; eauto. Qed.
+
+Lemma equiv_estep r0 a r1 :
+  r0 ==[, a ]==> r1 <-> estepf r0 = Some(a, r1).
+Proof.
+  (* FIXME: This proof is broken *)
+  (*
+  split.
+  - induction 1.
+    + (* ret *)
+      unfold estepf.
+      rewrite (get_rid_of_letstar (F, Ξ, E__foo :: ξ, H, Δ)).
+      rewrite elim_ectx_ret.
+      now rewrite (get_rid_of_letstar (E, Xreturn f)).
+    + (* call *)
+      unfold estepf.
+      rewrite (get_rid_of_letstar (F, Ξ, ξ, H, Δ)).
+      rewrite elim_ectx_call.
+      rewrite (get_rid_of_letstar (E, Xcall foo f)).
+      change ((fun o => (
+        match o with
+        | Some (argx0, _, e__foo0) =>
+            Some (Some (Scall foo f), (Some (F, Ξ, E :: ξ, H, Δ), Xreturn (subst argx0 e__foo0 f)))
+        | None => None
+        end = Some (Some (Scall foo f), (Some (F, Ξ, E :: ξ, H, Δ), Xreturn (subst argx e__foo f)))
+      )) (mget Ξ foo)).
+      now rewrite <- H0.
+    + (* normal step *) assert (H':=H); eapply pstep_compat_weaken in H.
+      apply (@grab_ectx e0 K e H) in H0 as H0';
+      unfold estepf; rewrite H0'; rewrite equiv_pstep in H2;
+      rewrite (get_rid_of_letstar Ω). rewrite (get_rid_of_letstar (K, e)).
+      inv H'. rewrite (get_rid_of_letstar e);
+      rewrite H2; rewrite (get_rid_of_letstar (a, (Some Ω', e')));
+      destruct e; trivial; inv H4.
+    + (* crash *) assert (H':=H); eapply pstep_compat_weaken in H.
+      apply (@grab_ectx e0 K e H) in H0 as H0'.
+      unfold estepf; rewrite H0'; rewrite equiv_pstep in H1;
+      rewrite (get_rid_of_letstar Ω). rewrite (get_rid_of_letstar (K, e)).
+      inv H'. rewrite (get_rid_of_letstar e);
+      rewrite H1; destruct e; trivial; inv H3.
+  - destruct r0 as [Ω e], r1 as [Ω' e'].
+    intros H; unfold estepf in H.
+    destruct Ω as [Ω|].
+    destruct (option_dec (evalctx_of_expr e)) as [Hx0 | Hy0]; try rewrite Hy0 in H.
+    2,3: inv H.
+    rewrite (get_rid_of_letstar Ω) in H.
+    apply not_eq_None_Some in Hx0 as [[K e0] Hx0].
+    rewrite Hx0 in H.
+    rewrite (get_rid_of_letstar (K, e0)) in H.
+    destruct (option_dec (pstep_compatible e0)) as [Hx1 | Hy1]; try rewrite Hy1 in H.
+    + apply not_eq_None_Some in Hx1 as [e0p Hx1].
+      rewrite Hx1 in H.
+      rewrite (get_rid_of_letstar e0p) in H.
+      destruct (option_dec (pstepf (Some Ω, e0))) as [Hx|Hy].
+      -- apply (not_eq_None_Some) in Hx as [[ap [oΩ' oe0']] Hx].
+         rewrite Hx in H.
+         rewrite (get_rid_of_letstar (ap, (oΩ', oe0'))) in H.
+         destruct oΩ' as [oΩ'|].
+         * apply pstep_compatible_some in Hx1 as Hx1'; subst.
+           destruct (e0p); try inversion Hx1;
+           assert (H':=H); inv H; eapply E_ctx; eauto using ungrab_ectx;
+           apply equiv_pstep; try eapply Hx.
+         * apply pstep_compatible_some in Hx1 as Hx1'; subst.
+           destruct e0p; try inversion Hx1; inv H;
+           eapply E_abrt_ctx; eauto using ungrab_ectx;
+           apply equiv_pstep in Hx; inv Hx; try apply e_abort.
+      -- rewrite Hy in H; inv H.
+         destruct e0; try congruence; inv Hx1.
+    + destruct e0; try congruence; inv Hy1; inv H.
+      * (* ret *)
+        grab_value e0.
+        -- destruct Ω as [[[[F Ξ] [|K__foo ξ]] H] Δ]; try congruence.
+           inv H1;
+           eapply ungrab_ectx in Hx0; subst; eauto using E_return.
+        -- destruct Ω as [[[[F Ξ] [|K__foo ξ]] H] Δ]; try congruence.
+           inv H1;
+           eapply ungrab_ectx in Hx0; subst; eauto using E_return.
+      * (* call *)
+        grab_value e0.
+        -- destruct Ω as [[[[F Ξ] ξ] H] Δ].
+           destruct (option_dec (mget Ξ foo)) as [Hx|Hy]; try (rewrite Hy in H1; congruence).
+          apply (not_eq_None_Some) in Hx as [[[x__arg τ__int] e__foo] Hx].
+           rewrite Hx in H1. inv H1.
+           eapply ungrab_ectx in Hx0; try rewrite Hx0; eauto.
+           eapply E_call; symmetry; eassumption.
+        -- destruct Ω as [[[[F Ξ] ξ] H] Δ].
+           destruct (option_dec (mget Ξ foo)) as [Hx|Hy]; try (rewrite Hy in H1; congruence).
+           apply (not_eq_None_Some) in Hx as [[[x__arg τ__int] e__foo] Hx].
+           rewrite Hx in H1. inv H1.
+           eapply ungrab_ectx in Hx0; subst; eauto.
+           eapply E_call; symmetry; eassumption.
+  *)
+Admitted.
+
+Lemma estepf_is_nodupinv_invariant Ω e Ω' e' a :
+  estepf (Ω ▷ e) = Some(a, Ω' ▷ e') ->
+  nodupinv Ω ->
+  nodupinv Ω'
+.
+Proof. intros H0 H1; apply equiv_estep in H0; apply estep_is_nodupinv_invariant in H0; eauto. Qed.
+
+(** Context splitting *)
+Reserved Notation "Γ '≡' Γ1 '∘' Γ2 '⊣' e" (at level 81, Γ1 at next level, Γ2 at next level, e at next level).
+Inductive splitting : Gamma -> Gamma -> Gamma -> expr -> Prop :=
+| splitEmpty : forall (e : expr), [⋅] ≡ [⋅] ∘ [⋅] ⊣ e
+| ℕsplit : forall (x : vart) (Γ Γ1 Γ2 : Gamma) (e : expr),
+    Γ ≡ Γ1 ∘ Γ2 ⊣ e ->
+    x ↦ (Texpr Tℕ) ◘ Γ ≡ x ↦ (Texpr Tℕ) ◘ Γ1 ∘ (x ↦ (Texpr Tℕ) ◘ Γ2) ⊣ e
+| weakPtrSplit : forall (x : vart) (Γ Γ1 Γ2 : Gamma) (e : expr),
+    Γ ≡ Γ1 ∘ Γ2 ⊣ e ->
+    x ↦ (Texpr Twptr) ◘ Γ ≡ x ↦ (Texpr Twptr) ◘ Γ1 ∘ (x ↦ (Texpr Twptr) ◘ Γ2) ⊣ e
+| ptrLSplit : forall (x : vart) (Γ Γ1 Γ2 : Gamma) (e : expr),
+    determine_pos x e = PosL ->
+    Γ ≡ Γ1 ∘ Γ2 ⊣ e ->
+    x ↦ (Texpr Tptr) ◘ Γ ≡ x ↦ (Texpr Tptr) ◘ Γ1 ∘ Γ2 ⊣ e
+| ptrRSplit : forall (x : vart) (Γ Γ1 Γ2 : Gamma) (e : expr),
+    determine_pos x e = PosR ->
+    Γ ≡ Γ1 ∘ Γ2 ⊣ e ->
+    x ↦ (Texpr Tptr) ◘ Γ ≡ x ↦ (Texpr Twptr) ◘ Γ1 ∘ (x ↦ (Texpr Tptr) ◘ Γ2) ⊣ e
+| ArrowSplit : forall (x : vart) (τ0 τ1 : ty) (Γ Γ1 Γ2 : Gamma) (e : expr),
+    int τ0 -> int τ1 ->
+    Γ ≡ Γ1 ∘ Γ2 ⊣ e ->
+    x ↦ (Tectx(Tarrow τ0 τ1)) ◘ Γ ≡ x ↦ (Tectx(Tarrow τ0 τ1)) ◘ Γ1 ∘ (x ↦ (Tectx(Tarrow τ0 τ1)) ◘ Γ2) ⊣ e
+where "Γ '≡' Γ1 '∘' Γ2 '⊣' e" := (splitting Γ Γ1 Γ2 e)
+.
+
+(** Typechecking *)
+Fixpoint NoOwnedPtr (Γ : Gamma) :=
+  match Γ with
+  | mapNil _ _ => True
+  | mapCons x τ Γ' => τ <> Tptr /\ NoOwnedPtr Γ'
+  end
+.
+Lemma noownedptr_cons Γ x τ :
+  NoOwnedPtr (x ↦ τ ◘ Γ) ->
+  NoOwnedPtr (x ↦ τ ◘ (mapNil _ _)) /\ NoOwnedPtr Γ
+.
+Proof. intros H; inv H; now repeat split. Qed.
+Lemma noownedptr_split Γ1 Γ2 :
+  NoOwnedPtr (Γ1 ◘ Γ2) <->
+  NoOwnedPtr Γ1 /\ NoOwnedPtr Γ2
+.
+Proof.
+  induction Γ1; cbn; split; intros H; try easy; fold (append Γ1 Γ2) in *.
+  - destruct H as [Ha Hb]. apply IHΓ1 in Hb as [Hb1 Hb2]; repeat split; auto.
+  - destruct H as [[Ha Hb] Hc]; split; trivial; apply IHΓ1; auto.
+Qed.
+
+Inductive check : VDash :=
+| CTvar : forall (x : vart) (Γ1 Γ2 : Gamma) (τ : Ty),
+    nodupinv (Γ1 ◘ x ↦ τ ◘ Γ2) ->
+    NoOwnedPtr Γ1 ->
+    NoOwnedPtr (x ↦ τ ◘ [⋅]) ->
+    NoOwnedPtr Γ2 ->
+    (Γ1 ◘ x ↦ τ ◘ Γ2) ⊦ Xres(Fvar x) : τ
+| CTℕ : forall (Γ : Gamma) (n : nat),
+    NoOwnedPtr Γ ->
+    Γ ⊦ Xres n : Tℕ
+| CToplus : forall (Γ1 Γ2 Γ3 : Gamma) (e1 e2 : expr) (b : binopsymb),
+    Γ3 ≡ Γ1 ∘ Γ2 ⊣ e1 ->
+    (Γ1 ⊦ e1 : (Texpr Tℕ)) ->
+    (Γ2 ⊦ e2 : (Texpr Tℕ)) ->
+    (Γ3 ⊦ Xbinop b e1 e2 : (Texpr Tℕ))
+| CTget : forall (Γ1 Γ2 Γ3 : Gamma) (x : vart) (e : expr),
+    Γ3 ≡ Γ1 ∘ Γ2 ⊣ (Fvar x) ->
+    (Γ2 ⊦ Xres(Fvar x) : (Texpr Twptr)) ->
+    (Γ1 ⊦ e : (Texpr Tℕ)) ->
+    (Γ3 ⊦ Xget x e : (Texpr Tℕ))
+| CTset : forall (Γ1 Γ2 Γ3 Γ12 Γ4 : Gamma) (x : vart) (e1 e2 : expr),
+    Γ12 ≡ Γ1 ∘ Γ2 ⊣ e1 ->
+    Γ4 ≡ Γ12 ∘ Γ3 ⊣ (Xbinop Badd e1 e2) ->
+    (Γ3 ⊦ (Xres(Fvar x)) : (Texpr Twptr)) ->
+    (Γ1 ⊦ e1 : (Texpr Tℕ)) ->
+    (Γ2 ⊦ e2 : (Texpr Tℕ)) ->
+    (Γ4 ⊦ Xset x e1 e2 : (Texpr Tℕ))
+| CTlet : forall (Γ1 Γ2 Γ3 : Gamma) (x : vart) (e1 e2 : expr) (τ1 τ2 : ty),
+    Γ3 ≡ Γ1 ∘ Γ2 ⊣ e1 ->
+    (Γ1 ⊦ e1 : (Texpr τ1)) ->
+    (x ↦ (Texpr τ1) ◘ Γ2 ⊦ e2 : (Texpr τ2)) ->
+    (Γ3 ⊦ Xlet x e1 e2 : (Texpr τ2))
+| CTnew : forall (Γ1 Γ2 Γ3 : Gamma) (x : vart) (e1 e2 : expr) (τ : ty),
+    Γ3 ≡ Γ1 ∘ Γ2 ⊣ e1 ->
+    (Γ1 ⊦ e1 : (Texpr Tℕ)) ->
+    (x ↦ (Texpr Tptr) ◘ Γ2 ⊦ e2 : (Texpr τ)) ->
+    (Γ3 ⊦ Xnew x e1 e2 : (Texpr τ))
+| CTdel : forall (Γ1 Γ2 : Gamma) (x : vart),
+    nodupinv (Γ1 ◘ x ↦ (Texpr Tptr) ◘ Γ2) ->
+    (Γ1 ◘ x ↦ (Texpr Tptr) ◘ Γ2 ⊦ Xdel x : (Texpr Tℕ))
+| CTcall : forall (Γ : Gamma) (foo : vart) (arg : expr) (τ0 τ1 : ty),
+    int τ0 -> int τ1 ->
+    (Γ ⊦ Xres(Fvar foo) : (Tectx(Tarrow τ0 τ1))) ->
+    (Γ ⊦ arg : (Texpr τ0)) ->
+    (Γ ⊦ Xcall foo arg : (Texpr τ1))
+| CTret : forall (Γ : Gamma) (e : expr) (τ : ty), (*TODO: intuitively, this should yield ⊥...?*)
+    int τ ->
+    (Γ ⊦ e : (Texpr τ)) ->
+    (Γ ⊦ Xreturn e : (Treturn τ))
+| CTifz : forall (Γ1 Γ2 Γ3 : Gamma) (c e1 e2 : expr) (τ : ty),
+    Γ3 ≡ Γ1 ∘ Γ2 ⊣ c ->
+    (Γ1 ⊦ c : (Texpr Tℕ)) ->
+    (Γ2 ⊦ e1 : (Texpr τ)) ->
+    (Γ2 ⊦ e2 : (Texpr τ)) ->
+    (Γ3 ⊦ Xifz c e1 e2 : (Texpr τ))
+.
+#[local]
+Hint Constructors check : core.
+
+(** splits Γ backtracking style. We do this, because input/output contexts have proven more difficult to reason about *)
+Fixpoint splitf (Γ : Gamma) (e : expr) : option (Gamma * Gamma) :=
+  match Γ with
+  | mapNil _ _ => (* splitEmpty *) Some([⋅], [⋅])
+  | mapCons x τ Γ' =>
+    match τ with
+    | Texpr τ__e =>
+      match τ__e with
+      | (Tℕ | Twptr) => (* ℕsplit, weakPtrSplit *)
+        let* (Γ1, Γ2) := splitf Γ' e in
+        Some(mapCons x τ Γ1, mapCons x τ Γ2)
+      | Tptr =>
+        let* (Γ1, Γ2) := splitf Γ' e in
+        match determine_pos x e with
+        | PosL => (* ptrLsplit *)
+          Some(mapCons x τ Γ1, Γ2)
+        | PosR => (* ptrRsplit *)
+          Some(mapCons x (Texpr Twptr) Γ1, mapCons x τ Γ2)
+        end
+      end
+    | Tarrow τ1 τ2 => (* ArrowSplit *)
+      let* _ := intf τ1 in
+      let* _ := intf τ2 in
+      let* (Γ1, Γ2) := splitf Γ' e in
+      Some(mapCons x τ Γ1, mapCons x τ Γ2)
+    | Treturn _ => None
+    end
+  end
+.
+Lemma splitf_sound (Γ Γ1 Γ2 : Gamma) (e : expr) :
+  splitf Γ e = Some(Γ1, Γ2) -> (Γ ≡ Γ1 ∘ Γ2 ⊣ e)
+.
+Proof.
+  revert Γ1 Γ2; induction Γ; intros Γ1 Γ2 H2; cbn in H2.
+  - someinv; constructor.
+  - destruct b; try congruence.
+    + destruct t; crush_option (splitf Γ e); try destruct x as [Γ1' Γ2']; someinv.
+      * constructor; now apply IHΓ.
+      * destruct q. remember (determine_pos a e) as q; symmetry in Heqq; destruct q; someinv.
+        -- constructor; auto.
+        -- constructor; auto.
+        -- someinv; constructor; now apply IHΓ.
+      * destruct q; now rewrite Hx in H2.
+    + destruct e0 as [τ1 τ2]; crush_intf τ1; crush_intf τ2; crush_option (splitf Γ e);
+      destruct x1 as [Γ1' Γ2']; someinv.
+      constructor; try now apply int_equiv_intf. now apply IHΓ.
+Qed.
+Lemma splitf_complete (Γ Γ1 Γ2 : Gamma) (e : expr) :
+  (Γ ≡ Γ1 ∘ Γ2 ⊣ e) ->
+  splitf Γ e = Some(Γ1, Γ2)
+.
+Proof.
+  induction 1; cbn; try easy.
+  - rewrite IHsplitting; easy.
+  - rewrite IHsplitting; easy.
+  - now rewrite IHsplitting, H.
+  - now rewrite IHsplitting, H.
+  - rewrite IHsplitting. now apply int_equiv_intf in H as ->; apply int_equiv_intf in H0 as ->.
+Qed.
+Lemma splitf_equiv_splitting (Γ Γ1 Γ2 : Gamma) (e : expr) :
+  splitf Γ e = Some(Γ1, Γ2) <-> (Γ ≡ Γ1 ∘ Γ2 ⊣ e)
+.
+Proof. split; eauto using splitf_complete, splitf_sound. Qed.
+
+Fixpoint noownedptrf (Γ : Gamma) : option Gamma :=
+  match Γ with
+  | mapNil _ _ => Some Γ
+  | mapCons x (Texpr τ) Γ' =>
+    let* _ := intf τ in
+    let* Γ'' := noownedptrf Γ' in
+    Some Γ
+  | mapCons x _ Γ' =>
+    let* Γ'' := noownedptrf Γ' in
+    Some Γ
+  end
+.
+Lemma noownedptrf_refl Γ Γ' :
+  noownedptrf Γ = Some Γ' -> Γ = Γ'
+.
+Proof.
+  revert Γ'; induction Γ; intros; inv H; try easy.
+  destruct b; inv H1.
+  - destruct (intf t); inv H0.
+    destruct (option_dec (noownedptrf Γ)) as [Hx | Hx]; try (rewrite Hx in H1; inv H1).
+    apply not_eq_None_Some in Hx as [x Hx]; rewrite Hx in H1.
+    now inv H1.
+  - destruct (option_dec (noownedptrf Γ)) as [Hx | Hx]; try (rewrite Hx in H0; inv H0).
+    apply not_eq_None_Some in Hx as [x Hx]; rewrite Hx in H0. now inv H0.
+  - destruct (option_dec (noownedptrf Γ)) as [Hx | Hx]; try (rewrite Hx in H0; inv H0).
+    apply not_eq_None_Some in Hx as [x Hx]; rewrite Hx in H0. now inv H0.
+Qed.
+Ltac crush_noownedptrf_aux Γ :=
+  let Hx' := fresh "Hx'" in
+  let Hx := fresh "Hx" in
+  let x := fresh "x" in
+  destruct (option_dec (noownedptrf Γ)) as [Hx | Hx];
+  try (rewrite Hx in *; congruence);
+  try (apply not_eq_None_Some in Hx as [x Hx]; eapply noownedptrf_refl in Hx as Hx'; rewrite <- Hx' in Hx; clear Hx'; rewrite Hx in *)
+.
+Lemma noownedptr_equiv_noownedptrf Γ :
+  NoOwnedPtr Γ <-> noownedptrf Γ = Some Γ
+.
+Proof.
+  induction Γ; cbn; split; intros H; try easy.
+  - destruct b; destruct H as [Ha Hb].
+    + crush_intf t.
+      * apply IHΓ in Hb. now rewrite Hb.
+      * apply int_equiv_intf_none in Hx.
+        exfalso; apply Hx. destruct t; try congruence; try constructor. destruct q; try constructor; contradiction.
+    + now apply IHΓ in Hb as ->.
+    + now apply IHΓ in Hb as ->.
+  - destruct b; crush_noownedptrf_aux Γ.
+    + crush_intf t. destruct t; inv Hx; split; try apply IHΓ; try easy; destruct q; easy.
+    + crush_intf t. rewrite Hx in H. inv H.
+    + destruct e; split; try apply IHΓ; easy.
+    + split; try apply IHΓ; easy.
+Qed.
+Ltac crush_noownedptrf Γ :=
+  crush_noownedptrf_aux Γ;
+  try (match goal with
+  | [H0: NoOwnedPtr ?Γ1, H1: NoOwnedPtr (?x ↦ ?τ ◘ [⋅]), H2: NoOwnedPtr ?Γ2 |- _] =>
+    let H01 := fresh "H01" in
+    let H012 := fresh "H012" in
+    assert (NoOwnedPtr Γ1 /\ NoOwnedPtr (x ↦ τ ◘ [⋅])) as H01%noownedptr_split by now split
+  end;
+  match goal with
+  | [H0: NoOwnedPtr (?Γ1 ◘ ?x ↦ ?τ ◘ [⋅]), H2: NoOwnedPtr ?Γ2 |- _] =>
+    let H012 := fresh "H012" in
+    assert (NoOwnedPtr (Γ1 ◘ x ↦ τ ◘ [⋅]) /\ NoOwnedPtr Γ2) as H012%noownedptr_split by now split
+  end;
+  match goal with
+  | [ H0: NoOwnedPtr ?Γ1, H1: NoOwnedPtr (?x ↦ ?τ ◘ [⋅]), H2: NoOwnedPtr ?Γ2,
+      H01: NoOwnedPtr (?Γ1 ◘ ?x ↦ ?τ ◘ [⋅]), H012: NoOwnedPtr ((?Γ1 ◘ ?x ↦ ?τ ◘ [⋅]) ◘ ?Γ2) |- _] =>
+    clear H0 H1 H2 H01; repeat rewrite append_assoc in H012; cbn in H012; apply noownedptr_equiv_noownedptrf in H012; congruence
+  end)
+.
+Definition inferf_var (Γ : Gamma) (x : vart) : option Ty :=
+  let* _ := undup Γ in
+  let* (Γ__a, _, τ, Γ__b) := splitat Γ x in
+  let* _ := noownedptrf Γ in
+  Some τ
+.
+
+Fixpoint inferf (Γ : Gamma) (e : expr) : option Ty :=
+  match e with
+  | Xres(Fres(Fvar x)) => inferf_var Γ x
+  | Xres(Fres(Fval(Vnat n))) =>
+    let* _ := noownedptrf Γ in
+    Some(Texpr Tℕ)
+  | Xbinop _ e1 e2 =>
+    let* (Γ1, Γ2) := splitf Γ e1 in
+    let* τ1 := inferf Γ1 e1 in
+    let* τ2 := inferf Γ2 e2 in
+    match τ1, τ2 with
+    | Texpr Tℕ, Texpr Tℕ => Some(Texpr Tℕ)
+    | _, _ => None
+    end
+  | Xdel x =>
+    let* _ := undup Γ in
+    let* (Γ1, y, τ, Γ2) := splitat Γ x in
+    match τ with
+    | Texpr Tptr => Some(Texpr Tℕ)
+    | _ => None
+    end
+  | Xcall foo arg =>
+    let* τ__f := inferf_var Γ foo in
+    let* τ0' := inferf Γ arg in
+    match τ0', τ__f with
+    | Texpr τ0__e', Tectx(Tarrow τ0 τ1) =>
+      let* _ := intf τ0 in
+      let* _ := intf τ1 in
+      if ty_eqb τ0 τ0__e' then
+        Some(Texpr τ1)
+      else
+        None
+    | _, _ => None
+    end
+  | Xreturn e' =>
+    let* τ := inferf Γ e' in
+    match τ with
+    | Texpr τ' =>
+      let* _ := intf τ' in
+      Some(Treturn τ')
+    | _ => None
+    end
+  | Xifz c e1 e2 =>
+    let* (Γ1, Γ2) := splitf Γ c in
+    let* τ__c := inferf Γ1 c in
+    let* τ1 := inferf Γ2 e1 in
+    let* τ2 := inferf Γ2 e2 in
+    match τ__c, τ1, τ2 with
+    | Texpr Tℕ, Texpr τ1', Texpr τ2' => if eq τ1' τ2' then Some(Texpr τ1') else None
+    | _, _, _ => None
+    end
+  | Xget x e' =>
+    let* (Γ1, Γ2) := splitf Γ (Fvar x) in
+    let* τ__x := inferf_var Γ2 x in
+    let* τ__e := inferf Γ1 e' in
+    match τ__x, τ__e with
+    | Texpr Twptr, Texpr Tℕ => Some(Texpr Tℕ)
+    | _, _ => None
+    end
+  | Xset x e1 e2 =>
+    let* (Γ12, Γ3) := splitf Γ (Xbinop Badd e1 e2) in
+    let* (Γ1, Γ2) := splitf Γ12 e1 in
+    let* τ1 := inferf Γ1 e1 in
+    let* τ2 := inferf Γ2 e2 in
+    let* τ3 := inferf_var Γ3 x in
+    match τ1, τ2, τ3 with
+    | Texpr Tℕ, Texpr Tℕ, Texpr Twptr => Some(Texpr Tℕ)
+    | _, _, _ => None
+    end
+  | Xlet x e1 e2 =>
+    let* (Γ1, Γ2) := splitf Γ e1 in
+    let* τ1 := inferf Γ1 e1 in
+    let* τ2 := inferf (x ↦ τ1 ◘ Γ2) e2 in
+    match τ1, τ2 with
+    | Texpr _, Texpr _ => Some τ2
+    | _, _ => None
+    end
+  | Xnew x e1 e2 =>
+    let* (Γ1, Γ2) := splitf Γ e1 in
+    let* τ1 := inferf Γ1 e1 in
+    let* τ2 := inferf (x ↦ (Texpr Tptr) ◘ Γ2) e2 in
+    match τ1, τ2 with
+    | Texpr Tℕ, Texpr _ => Some τ2
+    | _, _ => None
+    end
+  | _ => None
+  end
+.
+Lemma checkf_refinement (Γ : Gamma) (e : expr) (τ : Ty) :
+  inferf Γ e = Some τ ->
+  check Γ e τ
+.
+Proof.
+  revert Γ τ; induction e; intros Γ τ H0; cbn in H0.
+  - destruct f as [[]|].
+    + (* value *) destruct v. crush_noownedptrf Γ. someinv. constructor. now apply noownedptr_equiv_noownedptrf.
+    + (* variable *) crush_undup Γ; apply nodupinv_equiv_undup in Hx.
+      recognize_split; elim_split.
+      crush_noownedptrf (m1 ◘ v ↦ v0 ◘ m2). someinv. apply noownedptr_equiv_noownedptrf in Hx0.
+      apply noownedptr_split in Hx0 as [Hx0__a Hx0__b]. apply noownedptr_cons in Hx0__b as [Hx0__b Hx0__c].
+      constructor; auto.
+    + (* abort *) congruence.
+  - (* binop *) crush_option (splitf Γ e1); destruct x as [Γ1 Γ2].
+    crush_option (inferf Γ1 e1); crush_option (inferf Γ2 e2).
+    destruct x as [[]| |]; try congruence; destruct x0 as [[]| |]; try congruence; someinv.
+    specialize (IHe1 Γ1 _ Hx0) as IHe1'; specialize (IHe2 Γ2 _ Hx1).
+    erewrite splitf_equiv_splitting in Hx; eauto.
+    eapply CToplus; eauto.
+  - (* get *) crush_option (splitf Γ (Fvar x)); destruct x0 as [Γ1 Γ2].
+    crush_undup Γ2. apply nodupinv_equiv_undup in Hx0.
+    recognize_split; elim_split; crush_noownedptrf (m1 ◘ x ↦ v ◘ m2).
+    crush_option (inferf Γ1 e); destruct v as [[]| |]; try congruence; destruct q; try congruence.
+    destruct x2 as [[]| |]; try congruence; someinv.
+    eapply splitf_equiv_splitting in Hx; eauto.
+    eapply CTget; eauto. constructor; apply noownedptr_equiv_noownedptrf in Hx1;
+    apply noownedptr_split in Hx1 as [Hx1__a Hx1__b]; apply noownedptr_cons in Hx1__b as [Hx1__b Hx1__c]; auto.
+    eapply IHe; eauto.
+  - (* set *) crush_option (splitf Γ (Xbinop Badd e1 e2)); destruct x0 as [Γ12 Γ3].
+    crush_option (splitf Γ12 e1); destruct x0 as [Γ1 Γ2].
+    crush_option (inferf Γ1 e1); crush_option (inferf Γ2 e2). crush_undup Γ3.
+    apply nodupinv_equiv_undup in Hx3; recognize_split; elim_split.
+    crush_noownedptrf (m1 ◘ x ↦ v ◘ m2). destruct x0; try congruence; destruct t; try congruence.
+    destruct x1; try congruence; destruct t; try congruence. destruct v; try congruence; destruct t; try congruence.
+    destruct q; try congruence; someinv.
+    eapply splitf_equiv_splitting in Hx, Hx0. eapply CTset; eauto; try now (eapply IHe1 + eapply IHe2).
+    constructor; apply noownedptr_equiv_noownedptrf in Hx4;
+    apply noownedptr_split in Hx4 as [Hx4__a Hx4__b]; apply noownedptr_cons in Hx4__b as [Hx4__b Hx4__c]; auto.
+  - (* let *) crush_option (splitf Γ e1); destruct x0 as [Γ1 Γ2].
+    crush_option (inferf Γ1 e1); crush_option (inferf (x ↦ x0 ◘ Γ2) e2). destruct x0; try congruence.
+    destruct x1; try congruence; someinv. eapply splitf_equiv_splitting in Hx.
+    econstructor; eauto. eapply IHe1; eassumption. eapply IHe2; eassumption.
+  - (* new *) crush_option (splitf Γ e1); destruct x0 as [Γ1 Γ2].
+    crush_option (inferf Γ1 e1); crush_option (inferf (x ↦ (Texpr Tptr) ◘ Γ2) e2). destruct x0; try congruence.
+    destruct x1; try congruence; destruct t; try congruence. someinv. eapply splitf_equiv_splitting in Hx.
+    econstructor; eauto. eapply IHe1; eassumption. eapply IHe2; eassumption.
+  - (* del *) crush_undup Γ; apply nodupinv_equiv_undup in Hx.
+    recognize_split; elim_split. subst. destruct v as [[]| |]; try congruence. destruct q; try congruence.
+    someinv; constructor; easy.
+  - (* ret *) crush_option (inferf Γ e); destruct x; try congruence; someinv.
+    crush_intf t; someinv. constructor. now apply int_equiv_intf. now eapply IHe.
+  - (* call *) crush_undup Γ; eapply nodupinv_equiv_undup in Hx.
+    recognize_split; elim_split; crush_noownedptrf (m1 ◘ foo ↦ v ◘ m2).
+    crush_option (inferf (m1 ◘ foo ↦ v ◘ m2) e).
+    destruct x1; try congruence. destruct v; try congruence. destruct e0; try congruence.
+    crush_intf t0; crush_intf t1. destruct (eq_dec t0 t); subst; try (apply ty_eqb_neq in H1; rewrite H1 in H0; congruence).
+    rewrite ty_eqb_refl in H0; someinv. apply int_equiv_intf in Hx2, Hx3.
+    eapply CTcall. exact Hx2. exact Hx3.
+    apply noownedptr_equiv_noownedptrf in Hx0; apply noownedptr_split in Hx0 as [Hx0__a Hx0__b];
+    apply noownedptr_cons in Hx0__b as [Hx0__b Hx0__c]; eauto.
+    eapply IHe; eauto.
+  - (* ifz *) crush_option (splitf Γ e1); destruct x as [Γ1 Γ2].
+    crush_option (inferf Γ1 e1); crush_option (inferf Γ2 e2); crush_option (inferf Γ2 e3).
+    destruct x; try congruence. destruct t; try congruence. destruct x0, x1; try congruence.
+    destruct (eq_dec t t0); subst; try (apply ty_eqb_neq in H; rewrite H in H0; congruence).
+    rewrite ty_eqb_refl in H0; someinv. apply splitf_equiv_splitting in Hx; eapply CTifz; eauto;
+    try ((apply IHe1 + apply IHe2 + apply IHe3); eauto).
+  - (* abort *) congruence.
+Qed.
+
+Lemma checkf_correctness (Γ : Gamma) (e : expr) (τ : Ty) :
+  check Γ e τ ->
+  inferf Γ e = Some τ
+.
+Proof.
+  induction 1; cbn.
+  - (* CTvar *) crush_undup (Γ1 ◘ x ↦ τ ◘ Γ2); try (apply nodupinv_equiv_undup in H; congruence).
+    crush_option (splitat (Γ1 ◘ x ↦ τ ◘ Γ2) x); try (apply splitat_elim in H; congruence).
+    destruct x1 as [[[]]]; crush_noownedptrf (Γ1 ◘ x ↦ τ ◘ Γ2).
+    apply nodupinv_equiv_undup in Hx; apply splitat_elim in Hx; rewrite Hx in Hx0; someinv; reflexivity.
+  - (* CTℕ *) crush_noownedptrf Γ; auto; apply noownedptr_equiv_noownedptrf in H; congruence.
+  - (* CToplus *) crush_option (splitf Γ3 e1); apply (splitf_equiv_splitting _ _ _ e1) in H; try congruence.
+    destruct x as [Γ1' Γ2']; rewrite H in Hx; someinv.
+    now rewrite IHcheck, IHcheck0.
+  - (* CTget *) crush_option (splitf Γ3 (Fvar x)); apply (splitf_equiv_splitting _ _ _ (Fvar x)) in H; try congruence.
+    destruct x0 as [Γ1' Γ2']; rewrite H in Hx; someinv.
+    inv H0; crush_undup (Γ1 ◘ x ↦ (Texpr Twptr) ◘ Γ2).
+    apply nodupinv_equiv_undup in Hx; recognize_split; elim_split.
+    crush_noownedptrf (m1 ◘ x ↦ v ◘ m2); rewrite <- H0 in *; clear H0.
+    rewrite IHcheck0. apply splitat_elim in H3; rewrite H3 in H'; someinv; reflexivity.
+  - (* CTset *) crush_option (splitf Γ4 (Xbinop Badd e1 e2)); apply (splitf_equiv_splitting _ _ _ (Xbinop Badd e1 e2)) in H0; try congruence.
+    destruct x0 as [Γ12' Γ3']; rewrite H0 in Hx; someinv.
+    crush_option (splitf Γ12' e1); apply (splitf_equiv_splitting _ _ _ e1) in H; try congruence.
+    destruct x0 as [Γ1' Γ2']; rewrite H in Hx; someinv.
+    rewrite IHcheck0, IHcheck1. inv H1; crush_undup (Γ1 ◘ x ↦ (Texpr Twptr) ◘ Γ2).
+    apply nodupinv_equiv_undup in Hx; recognize_split; elim_split.
+    crush_noownedptrf (m1 ◘ x ↦ v ◘ m2); rewrite <- H1 in *; clear H1.
+    apply splitat_elim in H5; rewrite H5 in H'; someinv; reflexivity.
+  - (* CTlet *) crush_option (splitf Γ3 e1); apply (splitf_equiv_splitting _ _ _ e1) in H; try congruence.
+    destruct x0 as [Γ1' Γ2']; rewrite H in Hx; someinv. rewrite IHcheck, IHcheck0; reflexivity.
+  - (* CTnew *) crush_option (splitf Γ3 e1); apply (splitf_equiv_splitting _ _ _ e1) in H; try congruence.
+    destruct x0 as [Γ1' Γ2']; rewrite H in Hx; someinv. rewrite IHcheck, IHcheck0; reflexivity.
+  - (* CTdel *) crush_undup (Γ1 ◘ x ↦ (Texpr Tptr) ◘ Γ2); now apply splitat_elim in H as ->.
+  - (* CTcall *) inv H1; crush_undup (Γ1 ◘ foo ↦ (Tectx (Tarrow τ0 τ1)) ◘ Γ2).
+    recognize_split; elim_split. crush_noownedptrf (m1 ◘ foo ↦ v ◘ m2); rewrite <- H1 in *.
+    apply splitat_elim in H4; rewrite H4 in H'; rewrite IHcheck0; someinv.
+    apply int_equiv_intf in H as ->; apply int_equiv_intf in H0 as ->. now rewrite ty_eqb_refl.
+  - (* CTret *) rewrite IHcheck. now apply int_equiv_intf in H as ->.
+  - (* CTifz *) crush_option (splitf Γ3 c); apply (splitf_equiv_splitting _ _ _ c) in H; try congruence.
+    destruct x as [Γ1' Γ2']; rewrite H in Hx; someinv. rewrite IHcheck, IHcheck1, IHcheck0.
+    now rewrite ty_eqb_refl.
+Qed.
+
+Theorem checkf_equiv_check (Γ : Gamma) (e : expr) (τ : Ty) :
+  inferf Γ e = Some τ <-> (check Γ e τ)
+.
+Proof. split; now (eapply checkf_refinement + eapply checkf_correctness). Qed.
+
+
+Module ModAux <: CSC.Langs.Util.MOD.
+  Definition State := rtexpr.
+  Definition Ev := event.
+  Definition ev_eq := eventeq.
+  Definition step := estep.
+  Definition string_of_event := string_of_event.
+  Definition is_value := fun (r : rtexpr) => match r with
+                                          | (Some _, Xres(Fres _)) => true
+                                          | (_, _) => false
+                                          end.
+  Definition is_stuck := fun (r : rtexpr) => match r with
+                                          | (None, _) => True
+                                          | _ => False
+                                          end.
+End ModAux.
+Module SMod := CSC.Langs.Util.Mod(ModAux).
+Import SMod.
+
+Lemma different_reduction Ω Ω' e v v' As :
+  ((Ω ▷ e ==[As]==>* Ω' ▷ v) -> False) ->
+  Ω ▷ e ==[As]==>* Ω' ▷ v' ->
+  v <> v'
+.
+Proof.
+  intros H0 H1 H2; now subst.
+Qed.
+
+Lemma star_step_is_nodupinv_invariant Ω e Ω' e' As :
+  Ω ▷ e ==[ As ]==>* Ω' ▷ e' ->
+  nodupinv Ω ->
+  nodupinv Ω'
+.
+Proof.
+  assert (Some Ω = let (oΩ, e) := Ω ▷ e in oΩ) by easy;
+  assert (Some Ω' = let (oΩ', e') := Ω' ▷ e' in oΩ') by easy.
+  intros H__star; dependent induction H__star; try (inv H; inv H0; easy); try easy.
+  - destruct r2 as [[Ω2|] e2]; try (cbn in H0; contradiction); intros H__x;
+    eapply estep_is_nodupinv_invariant in H; eauto.
+  - destruct r2 as [[Ω2|] e2]; try (cbn in H0; contradiction); intros H__x;
+    eapply estep_is_nodupinv_invariant in H; eauto.
+Qed.
+
+(** Qualification to mark whether we go from context to component or vice versa *)
+Variant Qcall : Type :=
+| ctx_to_comp : Qcall
+| comp_to_ctx : Qcall
+.
+Definition Qcalleq (q1 q2 : Qcall) : bool :=
+  match q1, q2 with
+  | ctx_to_comp, ctx_to_comp => true
+  | comp_to_ctx, comp_to_ctx => true
+  | _, _ => false
+  end
+.
+(** Types of events that may occur in a trace. *)
+Variant fevent : Type :=
+| Sfalloc (ℓ : loc) (n : nat) : fevent
+| Sfdealloc (ℓ : loc) : fevent
+| Sfget (ℓ : loc) (n : nat) : fevent
+| Sfset (ℓ : loc) (n : nat) (v : value) : fevent
+| Sfcrash : fevent
+| Sfcall (q : Qcall) (foo : vart) (arg : fnoerr) : fevent
+| Sfret (q : Qcall) (f : fnoerr) : fevent
+.
+Definition feventeq (e1 e2 : fevent) : bool :=
+  match e1, e2 with
+  | Sfalloc(addr ℓ0) n0, Sfalloc(addr ℓ1) n1 => andb (Nat.eqb ℓ0 ℓ1) (Nat.eqb n0 n1)
+  | Sfdealloc(addr ℓ0), Sfdealloc(addr ℓ1) => Nat.eqb ℓ0 ℓ1
+  | Sfget(addr ℓ0) n0, Sfget(addr ℓ1) n1 => andb (Nat.eqb ℓ0 ℓ1) (Nat.eqb n0 n1)
+  | Sfset(addr ℓ0) n0 (Vnat v0), Sfset(addr ℓ1) n1 (Vnat v1) => andb (andb (Nat.eqb ℓ0 ℓ1) (Nat.eqb n0 n1))
+                                                                  (Nat.eqb v0 v1)
+  | Sfcrash, Sfcrash => true
+  | Sfcall q1 foo (Fval(Vnat v0)), Sfcall q2 bar (Fval(Vnat v1)) => andb (andb (String.eqb foo bar) (Nat.eqb v0 v1)) (Qcalleq q1 q2)
+  | Sfcall q1 foo (Fvar x), Sfcall q2 bar (Fvar y) => andb (andb (String.eqb foo bar) (String.eqb x y)) (Qcalleq q1 q2)
+  | Sfret q1 (Fval(Vnat v0)), Sfret q2 (Fval(Vnat v1)) => andb (Nat.eqb v0 v1) (Qcalleq q1 q2)
+  | Sfret q1 (Fvar x), Sfret q2 (Fvar y) => andb (String.eqb x y) (Qcalleq q1 q2)
+  | _, _ => false
+  end
+.
+#[local]
+Instance FEvent__Instance : TraceEvent fevent := {}.
+(** Pretty-printing function for better debuggability *)
+Definition string_of_fevent (e : fevent) := ""%string.
+
+(** Functional style version of star step from above. We need another parameter "fuel" to sidestep termination. *)
+Definition star_stepf (fuel : nat) (r : rtexpr) : option (tracepref * rtexpr) :=
+  let fix doo (fuel : nat) (r : rtexpr) :=
+    let (oΩ, e) := r in
+    let* Ω := oΩ in
+    match fuel, e with
+    | 0, Xres(Fres _) => (* refl *)
+      Some(nil, r)
+    | S fuel', _ => (* trans *)
+      let* (a, r') := estepf r in
+      let* (As, r'') := doo fuel' r' in
+      match a with
+      | None => Some(As, r'')
+      | Some(a') => Some(a' :: As, r'')
+      end
+    | _, _ => None
+    end
+  in doo fuel r
+.
+
+(** Finds the amount of fuel necessary to run an expression. *)
+Fixpoint get_fuel (e : expr) : option nat :=
+  match e with
+  | Xres _ => Some(0)
+  | Xbinop symb lhs rhs =>
+    let* glhs := get_fuel lhs in
+    let* grhs := get_fuel rhs in
+    Some(1 + glhs + grhs)
+  | Xget x e =>
+    let* ge := get_fuel e in
+    Some(1 + ge)
+  | Xset x e0 e1 =>
+    let* ge0 := get_fuel e0 in
+    let* ge1 := get_fuel e1 in
+    Some(1 + ge0 + ge1)
+  | Xlet x e0 e1 =>
+    let* ge0 := get_fuel e0 in
+    let* ge1 := get_fuel e1 in
+    Some(1 + ge0 + ge1)
+  | Xnew x e0 e1 =>
+    let* ge0 := get_fuel e0 in
+    let* ge1 := get_fuel e1 in
+    Some(1 + ge0 + ge1)
+  | Xdel x => Some(1)
+  | Xreturn e =>
+    match e with
+    | Xreturn e' => let* ge := get_fuel e' in Some(S ge)
+    | _ =>
+      let* ge := get_fuel e in
+      Some(1 + ge)
+    end
+  | Xcall foo e =>
+    let* ge := get_fuel e in
+    Some(1 + ge)
+  | Xifz c e0 e1 =>
+    let* gc := get_fuel c in
+    let* ge0 := get_fuel e0 in
+    let* ge1 := get_fuel e1 in
+    Some(1 + gc + ge0 + ge1)
+  | Xabort => Some(1)
+  end
+.
+Ltac crush_option :=
+    match goal with
+    | [H: Some _ = None |- _] => inv H
+    | [H: _ <> None |- _] =>
+      let n := fresh "n" in
+      apply (not_eq_None_Some) in H as [n H]
+    | [H: _ = None |- _] => trivial
+    end.
+Ltac crush_fuel := (match goal with
+| [H: Some _ = Some _ |- _] => inv H
+| [H: Some ?fuel = match (get_fuel ?e1) with Some _ => _ | None => None end |- _] =>
+  let Hx := fresh "Hx" in
+  let Hy := fresh "Hy" in
+  let n := fresh "n" in
+  destruct (option_dec (get_fuel e1)) as [Hx|Hy];
+  crush_option; try rewrite Hx in *; try rewrite Hy in *
+end).
+
+Lemma atleast_once Ω e r a fuel :
+  Some fuel = get_fuel e ->
+  Ω ▷ e ==[, a ]==> r ->
+  exists fuel', fuel = S fuel'.
+Proof.
+  revert fuel; induction e; cbn; intros fuel H; intros Ha.
+  - crush_fuel; crush_estep.
+  - repeat (crush_fuel + crush_option); now exists (n0 + n1).
+  - crush_fuel; try crush_option; exists n0; now inv H.
+  - repeat (crush_fuel + crush_option); now exists (n0 + n1).
+  - repeat (crush_fuel + crush_option); now exists (n0 + n1).
+  - repeat (crush_fuel + crush_option); now exists (n0 + n1).
+  - crush_fuel; now exists 0.
+  - destruct e; crush_fuel; try crush_option; exists n0; now inv H.
+  - crush_fuel; try crush_option; exists n0; now inv H.
+  - repeat (crush_fuel + crush_option); now exists (n0 + n1 + n2).
+  - exists 0; now inv H.
+Qed.
+Lemma star_stepf_one_step Ω e r r' a As fuel :
+  Some (S fuel) = get_fuel e ->
+  estep (Ω ▷ e) (Some a) r ->
+  star_stepf fuel r = Some(As, r') ->
+  star_stepf (S fuel) (Ω ▷ e) = Some(a :: As, r')
+.
+Proof. Admitted.
+Lemma star_stepf_one_unimportant_step Ω e r r' As fuel :
+  Some (S fuel) = get_fuel e ->
+  Ω ▷ e ==[]==> r ->
+  star_stepf fuel r = Some(As, r') ->
+  star_stepf (S fuel) (Ω ▷ e) = Some(As, r')
+.
+Proof. Admitted.
+Lemma estep_good_fuel Ω e r a fuel :
+  Some(S fuel) = get_fuel e ->
+  Ω ▷ e ==[, a ]==> r ->
+  Some fuel = get_fuel (let '(_, e') := r in e').
+Proof. Admitted.
+Lemma fuel_step oΩ e a oΩ' e' fuel :
+  Some(S fuel) = get_fuel e ->
+  (oΩ, e) ==[, a ]==> (oΩ', e') ->
+  Some fuel = get_fuel e'.
+Proof. Admitted.
+Lemma equiv_starstep Ω e r1 As fuel :
+  Some fuel = get_fuel e ->
+  Ω ▷ e ==[ As ]==>* r1 <-> star_stepf fuel (Ω ▷ e) = Some(As, r1).
+Proof.
+  intros Hf; split; intros H.
+  - destruct r1 as [oΩ' e'].
+    change (Some fuel = get_fuel match (Ω ▷ e) with
+                          | (_, e') => e'
+                          end) in Hf.
+    revert fuel Hf; induction H; intros fuel Hf; cbn in Hf.
+    + destruct r1 as [[Ω0|] e0]; cbn in *; try congruence.
+      destruct e0; cbn in H; try congruence; destruct f; try congruence.
+      inv Hf; now cbn.
+    + clear Ω e oΩ' e'; destruct r1 as [[oΩ1|] e1].
+      * assert (H':=H); apply (@atleast_once oΩ1 e1 r2 (Some a) fuel Hf) in H as [fuel' ->];
+        eapply star_stepf_one_step; eauto;
+        eapply IHstar_step; eapply estep_good_fuel; eauto.
+      * inv H.
+    + clear Ω e oΩ' e'; destruct r1 as [[oΩ1|] e1].
+      * assert (H':=H); apply (@atleast_once oΩ1 e1 r2 None fuel Hf) in H as [fuel' ->].
+        eapply star_stepf_one_unimportant_step; eauto;
+        eapply IHstar_step; eapply estep_good_fuel; eauto.
+      * inv H.
+  - revert Ω e r1 As Hf H; induction fuel; intros Ω e r1 As Hf H.
+    + destruct e; cbn in Hf; repeat destruct (get_fuel _); try congruence;
+      cbn in H; inv H; destruct f; try congruence; inv H1; now apply ES_refl.
+    + unfold star_stepf in H.
+      rewrite (get_rid_of_letstar Ω) in H.
+      destruct (option_dec (estepf (Some Ω, e))) as [Hx|Hy]; try rewrite Hy in H.
+      2: inv H.
+      apply not_eq_None_Some in Hx as [[a [Ω' e']] Hx].
+      rewrite Hx in H.
+      rewrite (get_rid_of_letstar (a, (Ω', e'))) in H.
+      destruct (option_dec ((
+fix doo (fuel : nat) (r : rtexpr) {struct fuel} : option (list event * rtexpr) :=
+            let (oΩ, e) := r in
+            let* _ := oΩ
+            in match fuel with
+               | 0 => match e with
+                      | Xres(Fres _) => Some (nil, r)
+                      | _ => None
+                      end
+               | S fuel' =>
+                   let* (a, r') := estepf r
+                   in let* (As, r'') := doo fuel' r'
+                      in match a with
+                         | Some a' => Some (a' :: As, r'')
+                         | None => Some (As, r'')
+                         end
+               end
+                ) fuel (Ω', e'))) as [Hx0|Hy0]; try rewrite Hy0 in H.
+      2: inv H.
+      apply not_eq_None_Some in Hx0 as [[As0 r1'] Hx0].
+      rewrite Hx0 in H.
+      rewrite (get_rid_of_letstar (As0, r1')) in H.
+      rewrite <- equiv_estep in Hx;
+      destruct a as [a|]; inv H.
+      * eapply ES_trans_important; eauto;
+        destruct Ω' as [Ω'|]; try now cbn.
+        1,3: destruct fuel; inv Hx0.
+        apply (fuel_step Hf) in Hx.
+        eapply IHfuel; eauto.
+      * eapply ES_trans_unimportant; eauto;
+        destruct Ω' as [Ω'|]; try now cbn.
+        apply (fuel_step Hf) in Hx.
+        eapply IHfuel; eauto.
+Qed.
+
+Lemma star_stepf_is_nodupinv_invariant Ω e Ω' e' a fuel :
+  Some fuel = get_fuel e ->
+  star_stepf fuel (Ω ▷ e) = Some(a, Ω' ▷ e') ->
+  nodupinv Ω ->
+  nodupinv Ω'
+.
+Proof. intros H__fuel H0 H1; apply equiv_starstep in H0; eauto; apply star_step_is_nodupinv_invariant in H0; eauto. Qed.
+
+(** Evaluation of programs *)
+Inductive wstep : prog -> tracepref -> rtexpr -> Prop :=
+| e_wprog : forall (symbs : symbols) (ξ : commlib) (As : tracepref) (r : rtexpr),
+    prog_check (Cprog symbs ξ) ->
+    (Fresh.empty_fresh ; symbs ; ξ ; nil ; hNil ; sNil ▷ Xcall "main"%string 0 ==[ As ]==>* r) ->
+    wstep (Cprog symbs ξ) As r
+.
+
+Fixpoint get_fuel_fn_aux (E : evalctx) {struct E} : option nat :=
+  match E with
+  | Khole => Some 0
+  | KbinopL b K e =>
+    let* gK := get_fuel_fn_aux K in
+    let* ge := get_fuel e in
+    Some(ge + gK + 1)
+  | KbinopR b v K =>
+    let* gK := get_fuel_fn_aux K in
+    Some(gK + 1)
+  | Kget x K =>
+    let* gK := get_fuel_fn_aux K in
+    Some(gK + 1)
+  | KsetL x K e =>
+    let* gK := get_fuel_fn_aux K in
+    let* ge := get_fuel e in
+    Some(ge + gK + 1)
+  | KsetR x v K =>
+    let* gK := get_fuel_fn_aux K in
+    Some(gK + 1)
+  | Klet x K e =>
+    let* gK := get_fuel_fn_aux K in
+    let* ge := get_fuel e in
+    Some(ge + gK + 1)
+  | Knew x K e =>
+    let* gK := get_fuel_fn_aux K in
+    let* ge := get_fuel e in
+    Some(ge + gK + 1)
+  | Kifz K e0 e1 =>
+    let* gK := get_fuel_fn_aux K in
+    let* ge0 := get_fuel e0 in
+    let* ge1 := get_fuel e1 in
+    Some(ge0 + ge1 + gK + 1)
+  | Kreturn K =>
+    let* gK := get_fuel_fn_aux K in
+    Some(gK + 1)
+  | Kcall foo K =>
+    let* gK := get_fuel_fn_aux K in
+    Some(gK + 1)
+  end
+.
+Fixpoint get_fuel_fn (e : expr) : option nat :=
+  match e with
+  | Xres _ => Some 0
+  | Xabort | Xdel _ => Some 1
+  | Xbinop b e1 e2 =>
+    let* f1 := get_fuel_fn e1 in
+    let* f2 := get_fuel_fn e2 in
+    Some (f1 + f2 + 1)
+  | Xget x e' =>
+    let* f := get_fuel_fn e' in
+    Some (f + 1)
+  | Xset x e1 e2 =>
+    let* f1 := get_fuel_fn e1 in
+    let* f2 := get_fuel_fn e2 in
+    Some (f1 + f2 + 1)
+  | Xlet x e1 e2 =>
+    let* f1 := get_fuel_fn e1 in
+    let* f2 := get_fuel_fn e2 in
+    Some (f1 + f2 + 1)
+  | Xnew x e1 e2 =>
+    let* f1 := get_fuel_fn e1 in
+    let* f2 := get_fuel_fn e2 in
+    Some (f1 + f2 + 1)
+  | Xifz e0 e1 e2 =>
+    let* f0 := get_fuel_fn e0 in
+    let* f1 := get_fuel_fn e1 in
+    let* f2 := get_fuel_fn e2 in
+    Some (f0 + f1 + f2 + 1)
+  | Xreturn e' =>
+    let* f := get_fuel_fn e' in
+    Some (f + 1)
+  | Xcall foo e' =>
+    let* f := get_fuel_fn e' in
+    Some (f + 1)
+  end
+.
+Fixpoint collect_callsites (ξ : symbols) (e : expr) : option symbols :=
+  match e with
+  | Xbinop _ e0 e1 =>
+    let* r0 := collect_callsites ξ e0 in
+    let* r1 := collect_callsites ξ e1 in
+    Some(r0 ◘ r1)
+  | Xget _ e => collect_callsites ξ e
+  | Xset _ e0 e1 =>
+    let* r0 := collect_callsites ξ e0 in
+    let* r1 := collect_callsites ξ e1 in
+    Some(r0 ◘ r1)
+  | Xlet _ e0 e1 =>
+    let* r0 := collect_callsites ξ e0 in
+    let* r1 := collect_callsites ξ e1 in
+    Some(r0 ◘ r1)
+  | Xnew _ e0 e1 =>
+    let* r0 := collect_callsites ξ e0 in
+    let* r1 := collect_callsites ξ e1 in
+    Some(r0 ◘ r1)
+  | Xreturn e' => collect_callsites ξ e'
+  | Xcall foo e' =>
+    let* res := collect_callsites ξ e' in
+    let* K := mget ξ foo in
+    Some(foo ↦ K ◘ res)
+  | Xifz c e0 e1 =>
+    let* cr := collect_callsites ξ c in
+    let* r0 := collect_callsites ξ e0 in
+    let* r1 := collect_callsites ξ e1 in
+    Some(cr ◘ r0 ◘ r1)
+  | _ => Some(mapNil _ _)
+  end
+.
+(** Compute the total amount of fuel necessary to run a complete program. Each context corresponding to a call
+    artificially gets a return in the semantics (estep), so add 1.
+    Also, add 1 to the final result, because the top-level performs a call to "main". *)
+Definition get_fuel_toplevel (ξ : symbols) (foo : vart) : option nat :=
+  let* Kτ := mget ξ foo in
+  let '(x__arg,_,e__arg) := Kτ in
+  let e := subst x__arg e__arg (Xres 0) in
+  let* ge := get_fuel e in
+  let* symbs := collect_callsites ξ e in
+  let* res := List.fold_left (fun acc Eτ =>
+                                let '(_,_,e__arg) := Eτ in
+                                let* a := acc in
+                                let* b := get_fuel_fn e__arg in
+                                Some(1 + a + b)) (img symbs) (Some ge) in
+  Some(S res)
+.
+
+Definition wstepf (p : prog) : option (tracepref * rtexpr) :=
+  let '(Cprog symbs ξ) := p in
+  let e := Xcall "main"%string 0 in
+  let* fuel := get_fuel_toplevel symbs "main"%string in
+  let R := Fresh.empty_fresh ; symbs ; ξ ; nil ; hNil ; sNil ▷ e in
+  star_stepf fuel R
+.
+Definition debug_eval (p : prog) :=
+  let* (As, _) := wstepf p in
+  Some(string_of_tracepref As)
+.
+
+(* let x = [] in
+     let z = new x in
+     let w = z[1337] in
+     let _ = delete z in
+     w*)
+Definition smsunsafe_ep : expr :=
+  Xnew "z"%string
+      (Fvar "y"%string)
+      (Xlet "w"%string
+            (Xget "z"%string 1337)
+            (Xlet "_1"%string
+                  (Xdel "z"%string)
+                  (Fvar "w"%string))
+      )
+.
+(* let x = 3 in call foo x *)
+Definition smsunsafe_ctx : expr :=
+  Xreturn (Xlet ("_0"%string)
+    (Fvar "arg"%string)
+    (Xlet ("x"%string)
+          3
+          (Xcall ("foo"%string) (Fvar "x"%string))))
+.
+
+Definition smsunsafe_prog_aux : symbols :=
+  ("foo"%string ↦ ("y"%string, Tectx(Tarrow Tℕ Tℕ), smsunsafe_ep) ◘
+  ("main"%string ↦ ("arg"%string, Tectx(Tarrow Tℕ Tℕ), smsunsafe_ctx) ◘ mapNil _ _)).
+Definition smsunsafe_prog := Cprog smsunsafe_prog_aux ("foo"%string :: List.nil).
+
+Tactic Notation "splitΓfor" :=
+try do 2 match goal with
+| [|- _ ⊦ _ : _] => unfold "_ ⊦ _ : _"
+| [|- check ?P (Xdel ?x) ?τ] =>
+  match P with
+  | context E__Γ [(x ↦ ?H ◘ ?R)] =>
+    let nP := constr:([⋅] ◘ (x ↦ H ◘ R)) in
+    let NP := constr:(ltac:(let t := context E__Γ [[⋅]] in exact t)) in
+    let nnP := constr:(NP ◘ nP) in
+    let G := constr:(check nnP (Xdel x) τ) in
+    change G
+  end
+| [|- check ?P (Xres(Fres(Fvar ?x))) ?τ] =>
+  match P with
+  | context E__Γ [(x ↦ ?H ◘ ?R)] =>
+    let nP := constr:([⋅] ◘ (x ↦ H ◘ R)) in
+    let NP := constr:(ltac:(let t := context E__Γ [[⋅]] in exact t)) in
+    let nnP := constr:(NP ◘ nP) in
+    let G := constr:(check nnP (Xres(Fres(Fvar x))) τ) in
+    change G
+  end
+end.
+
+Lemma ownedptrsplit Γ1 Γ2 : NoOwnedPtr Γ1 -> NoOwnedPtr Γ2 -> NoOwnedPtr (Γ1 ◘ Γ2).
+Proof.
+  induction Γ1; cbn; intros H1 H2; trivial; destruct H1 as [H1__a H1__b]; auto.
+Qed.
+Lemma ownedptrcons x y Γ2 : NoOwnedPtr (x ↦ y ◘ [⋅]) -> NoOwnedPtr Γ2 -> NoOwnedPtr (x ↦ y ◘ Γ2).
+Proof.
+  intros [H1__a H1__b] H2; split; auto.
+Qed.
+
+Lemma smsunsafe_prog_checks : prog_check smsunsafe_prog.
+Proof.
+  (*
+  assert (NoOwnedPtr ("foo"%string ↦ (Tectx(Tarrow Tℕ Tℕ)) ◘ ("main"%string ↦ (Tectx(Tarrow Tℕ Tℕ)) ◘ [⋅]))) as G.
+    unfold NoOwnedPtr. intros. destruct x; cbn in H; inv H. destruct a.
+    destruct b, b0, b1, b2, b3, b4, b5, b6; inv H1; destruct x; inv H0;
+    destruct a; inv H1; destruct b, b0, b1, b2, b3, b4, b5, b6; inv H0;
+    destruct x; inv H1; destruct a; inv H0; destruct b, b0, b1, b2, b3, b4, b5, b6; inv H1;
+    destruct x; inv H0; destruct a; inv H1; destruct b, b0, b1, b2, b3, b4, b5, b6; inv H0.
+    destruct x; inv H1.
+  cbn; repeat split; trivial.
+  - eapply ETlet. repeat (eapply ArrowSplit; try eapply intℕ); eapply splitEmpty. eapply EThole.
+    eapply intℕ. exact G.
+    eapply CTnew. eapply ℕsplit, ArrowSplit, ArrowSplit, splitEmpty; try eapply intℕ.
+    splitΓfor.
+    eapply CTvar. easy. unfold NoOwnedPtr. intros. destruct x; cbn in H; inv H. destruct a.
+    destruct b, b0, b1, b2, b3, b4, b5, b6; inv H1. destruct x; inv H0. easy.
+    exact G.
+    eapply CTlet. eapply ptrRSplit, ℕsplit, ArrowSplit, ArrowSplit, splitEmpty; try eapply intℕ.
+    eapply CTget. eapply weakPtrSplit, ℕsplit, ArrowSplit, ArrowSplit, splitEmpty; try eapply intℕ.
+    splitΓfor.
+    eapply CTvar. easy. unfold NoOwnedPtr. intros. destruct x; cbn in H; inv H. destruct a.
+    destruct b, b0, b1, b2, b3, b4, b5, b6; inv H1. destruct x; inv H0. easy.
+    eapply ownedptrcons; trivial.
+    unfold NoOwnedPtr. intros. destruct x; cbn in H; inv H. destruct a.
+    destruct b, b0, b1, b2, b3, b4, b5, b6; inv H1. destruct x; inv H0. easy.
+    eapply CTℕ. do 2 eapply ownedptrcons; try easy.
+    unfold NoOwnedPtr. intros. destruct x; cbn in H; inv H. destruct a.
+    destruct b, b0, b1, b2, b3, b4, b5, b6; inv H1; destruct x; inv H0; easy.
+    unfold NoOwnedPtr. intros. destruct x; cbn in H; inv H. destruct a.
+    destruct b, b0, b1, b2, b3, b4, b5, b6; inv H1; destruct x; inv H0; easy.
+    eapply CTlet. eapply ℕsplit, ptrLSplit, ℕsplit, ArrowSplit, ArrowSplit, splitEmpty; eapply intℕ.
+    instantiate (1:=Tℕ).
+    splitΓfor.
+    eapply CTdel.
+    splitΓfor.
+    eapply CTvar.
+    unfold NoOwnedPtr. intros. destruct x; cbn in H; inv H. destruct a.
+    destruct b, b0, b1, b2, b3, b4, b5, b6; inv H1; destruct x; inv H0.
+    destruct a. destruct b, b0, b1, b2, b3, b4, b5, b6; inv H1. destruct x; inv H0. easy.
+    unfold NoOwnedPtr. intros. destruct x; cbn in H; inv H. destruct a.
+    destruct b, b0, b1, b2, b3, b4, b5, b6; inv H1; destruct x; inv H0; easy.
+    eapply ownedptrcons; try easy.
+    unfold NoOwnedPtr. intros. destruct x; cbn in H; inv H. destruct a.
+    destruct b, b0, b1, b2, b3, b4, b5, b6; inv H1; destruct x; inv H0; easy.
+  - eapply ETret. eapply intℕ. eapply ETlet. eapply ArrowSplit, ArrowSplit, splitEmpty; eapply intℕ.
+    eapply EThole. eapply intℕ. assumption.
+    eapply CTlet. eapply ℕsplit, ArrowSplit, ArrowSplit, splitEmpty; eapply intℕ. eapply CTℕ.
+    eapply ownedptrcons; try easy.
+    unfold NoOwnedPtr. intros. destruct x; cbn in H; inv H. destruct a.
+    destruct b, b0, b1, b2, b3, b4, b5, b6; inv H1; destruct x; inv H0.
+    destruct a; destruct b, b0, b1, b2, b3, b4, b5, b6; inv H1. destruct x; inv H0; easy.
+    eapply CTcall. eapply intℕ. eapply intℕ.
+    splitΓfor. eapply CTvar; try easy.
+    unfold NoOwnedPtr. intros. destruct x; cbn in H; inv H. destruct a.
+    destruct b, b0, b1, b2, b3, b4, b5, b6; inv H1; destruct x; inv H0.
+    destruct a. destruct b, b0, b1, b2, b3, b4, b5, b6; inv H1; destruct x; inv H0; easy. easy.
+    unfold NoOwnedPtr. intros. destruct x; cbn in H; inv H. destruct a.
+    destruct b, b0, b1, b2, b3, b4, b5, b6; inv H1; destruct x; inv H0.
+    destruct a; destruct b, b0, b1, b2, b3, b4, b5, b6; inv H1. destruct x; inv H0.
+    destruct a; destruct b, b0, b1, b2, b3, b4, b5, b6; inv H1. destruct x; easy.
+    unfold NoOwnedPtr. intros. destruct x; cbn in H; inv H. destruct a.
+    destruct b, b0, b1, b2, b3, b4, b5, b6; inv H1; destruct x; inv H0.
+    destruct a.
+    destruct b, b0, b1, b2, b3, b4, b5, b6; inv H1; destruct x; inv H0.
+    destruct a.
+    destruct b, b0, b1, b2, b3, b4, b5, b6; inv H1; destruct x; inv H0.
+    destruct a.
+    destruct b, b0, b1, b2, b3, b4, b5, b6; inv H1; destruct x; inv H0.
+    splitΓfor.
+    eapply CTvar. easy.
+    unfold NoOwnedPtr. intros. destruct x; cbn in H; inv H. destruct a.
+    destruct b, b0, b1, b2, b3, b4, b5, b6; inv H1; destruct x; inv H0; easy.
+    eapply ownedptrcons; try easy.
+    unfold NoOwnedPtr. intros. destruct x; cbn in H; inv H. destruct a.
+    destruct b, b0, b1, b2, b3, b4, b5, b6; inv H1; destruct x; inv H0.
+    destruct a. destruct b, b0, b1, b2, b3, b4, b5, b6; inv H1; destruct x; inv H0; easy.
+    *)
+Admitted.
+
+Goal exists As R,
+    wstep smsunsafe_prog As R.
+Proof.
+  (*
+  do 2 eexists.
+  econstructor; try exact smsunsafe_prog_checks.
+  econstructor 2. rewrite equiv_estep; now cbn. now cbn.
+  econstructor 3. rewrite equiv_estep; now cbn. now cbn.
+  econstructor 3. rewrite equiv_estep; now cbn. now cbn.
+  econstructor 2. rewrite equiv_estep; now cbn. now cbn.
+  econstructor 3. rewrite equiv_estep; now cbn. now cbn.
+  econstructor 2. rewrite equiv_estep; now cbn. now cbn.
+  econstructor 2. rewrite equiv_estep; now cbn. now cbn.
+  econstructor 3. rewrite equiv_estep; now cbn. now cbn.
+  econstructor 2. rewrite equiv_estep; now cbn. now cbn.
+  econstructor 3. rewrite equiv_estep; now cbn. now cbn.
+  econstructor 2. rewrite equiv_estep; now cbn. now cbn.
+  econstructor 2. rewrite equiv_estep; now cbn. now cbn.
+  now econstructor. *)
+Admitted.
+
+Compute (debug_eval smsunsafe_prog).
+
+Variant msevent : Type :=
+| MSalloc (ℓ : loc) (n : nat) : msevent
+| MSdealloc (ℓ : loc) : msevent
+| MSuse (ℓ : loc) (n : nat) : msevent
+| MScrash : msevent
+.
+#[local]
+Instance msevent__Instance : TraceEvent msevent := {}.
+Definition mseventeq (e1 e2 : msevent) : bool :=
+  match e1, e2 with
+  | MSalloc(addr ℓ0) n0, MSalloc(addr ℓ1) n1 => andb (Nat.eqb ℓ0 ℓ1) (Nat.eqb n0 n1)
+  | MSdealloc(addr ℓ0), MSdealloc(addr ℓ1) => Nat.eqb ℓ0 ℓ1
+  | MSuse(addr ℓ0) n0, MSuse(addr ℓ1) n1 => andb (Nat.eqb ℓ0 ℓ1) (Nat.eqb n0 n1)
+  | MScrash, MScrash => true
+  | _, _ => false
+  end
+.
+(** Pretty-printing function for better debuggability *)
+Definition string_of_msevent (e : msevent) :=
+  match e with
+  | (MSalloc (addr ℓ) n) => String.append
+                      (String.append ("MsAlloc ℓ"%string) (string_of_nat ℓ))
+                      (String.append (" "%string) (string_of_nat n))
+  | (MSdealloc (addr ℓ)) => String.append ("MsDealloc ℓ"%string) (string_of_nat ℓ)
+  | (MSuse (addr ℓ) n) => String.append
+                    (String.append ("MsUse ℓ"%string) (string_of_nat ℓ))
+                    (String.append (" "%string) (string_of_nat n))
+  | (MScrash) => "↯"%string
+  end
+.
+
+Module MSModAux <: CSC.Langs.Util.MOD.
+  Definition State := True.
+  Definition Ev := msevent.
+  Definition ev_eq := mseventeq.
+  Definition step := fun (_ : State) (o : option msevent) (_ : State) => True.
+  Definition string_of_event := string_of_msevent.
+  Definition is_value := fun (_ : State) => true.
+  Definition is_stuck := fun (_ : State) => False.
+End MSModAux.
+Module SMSMod := CSC.Langs.Util.Mod(MSModAux).
+
+Definition msev_of_ev (ev : event) : option msevent :=
+  match ev with
+  | Sstart | Send _ => None
+  | Salloc ℓ n => Some(MSalloc ℓ n)
+  | Sdealloc ℓ => Some(MSdealloc ℓ)
+  | Sget ℓ n => Some(MSuse ℓ n)
+  | Sset ℓ n _ => Some(MSuse ℓ n)
+  | Scrash => Some(MScrash)
+  | Scall _ _ _ => None
+  | Sret _ _ => None
+  end
+.
+Fixpoint mstracepref_of_tracepref (tr : tracepref) : SMSMod.tracepref :=
+  match tr with
+  | nil => nil
+  | a :: tr' =>
+    match msev_of_ev a with
+    | Some a' => a' :: (mstracepref_of_tracepref tr')
+    | None => mstracepref_of_tracepref tr'
+    end
+  end
+.
+
+Module TMMon := CSC.Langs.TMMon.
+Module TMMonM := TMMon.TMSMod.
+
+Definition deltamap := mapind loceq__Instance TMMon.loc.
+
+Lemma snodupinv_implies_δnodupinv Δ :
+  snodupinv Δ ->
+  Util.nodupinv (δ_of_Δ Δ)
+.
+Proof. induction 1; try constructor; destruct ℓ; constructor; trivial. Qed.
+
+(** Trace agreement between memory specific events and TMS monitor events. *)
+Inductive ev_eq (δ : deltamap) : option msevent -> option TMMon.event -> Prop :=
+| TMSAuthAlloc : forall ℓ ℓ' n, Util.nodupinv δ -> mget δ ℓ = Some ℓ' -> ev_eq δ (Some(MSalloc ℓ n)) (Some(TMMon.Salloc ℓ'))
+| TMSAuthDealloc : forall ℓ ℓ', Util.nodupinv δ -> mget δ ℓ = Some ℓ' -> ev_eq δ (Some(MSdealloc ℓ)) (Some(TMMon.Sdealloc ℓ'))
+| TMSAuthUse : forall ℓ ℓ' n, Util.nodupinv δ -> mget δ ℓ = Some ℓ' -> ev_eq δ (Some(MSuse ℓ n)) (Some(TMMon.Suse ℓ'))
+| TMSAuthNone : Util.nodupinv δ -> ev_eq δ (None) (None)
+.
+Inductive mstracepref_eq (δ : deltamap) : SMSMod.tracepref -> TMMonM.tracepref -> Prop :=
+| TMSAuthRefl : Util.nodupinv δ -> mstracepref_eq δ nil nil
+| TMSAuthTrans : forall a a' As As', ev_eq δ (Some a) (Some a') ->
+                                mstracepref_eq δ As As' ->
+                                mstracepref_eq δ (a :: As) (a' :: As')
+.
+
+Import TMMon.TMMonNotation.
+(** Store agreement between our stores and the TMS monitor. *)
+Inductive store_agree (δ : deltamap) : TMMon.TMSMonitor -> store -> Prop :=
+| EmptyAgree : Util.nodupinv δ -> store_agree δ TMMon.emptytmsmon sNil
+| ConsAgree : forall (x : vart) (ℓ : loc) (ℓ' : TMMon.loc) (T__TMS : TMMon.TMSMonitor) (Δ : store),
+    Util.nodupinv δ ->
+    mget δ ℓ = Some ℓ' ->
+    ℓ' ∉ T__TMS ->
+    store_agree δ T__TMS Δ ->
+    store_agree δ ({ℓ'} ∪ T__TMS) (x ↦ (ℓ ⋅ ◻) ◘ Δ)
+| PoisonAgree : forall (x : vart) (ℓ : loc) (ℓ' : TMMon.loc) (T__TMS : TMMon.TMSMonitor) (Δ : store),
+    Util.nodupinv δ ->
+    mget δ ℓ = Some ℓ' ->
+    store_agree δ T__TMS Δ ->
+    store_agree δ T__TMS (x ↦ (ℓ ⋅ ☣) ◘ Δ)
+.
+Inductive state_agree (δ : deltamap) : TMMon.TMSMonitor -> state -> Prop :=
+| StateAgree : forall F Ξ ξ K H Δ T__TMS, store_agree δ T__TMS Δ -> state_agree δ T__TMS (F ; Ξ ; ξ ; K ; H ; Δ)
+.
+
+Definition TMS (As : tracepref) :=
+  forall MAs : SMSMod.tracepref, MAs = mstracepref_of_tracepref As ->
+                            exists δ (Bs : TMMonM.tracepref), mstracepref_eq δ MAs Bs /\
+                                                         TMMon.TMS Bs
+.
+
+Definition substτ (Γ : Gamma) (what fore : vart) :=
+  match Γ with
+  | mapNil _ _ => mapNil _ _
+  | mapCons x t Γ' =>
+    if vareq x what then
+      mapCons fore t Γ'
+    else
+      mapCons x t Γ'
+  end
+.
+
+(** Store splitting. We don't need a case for nat, since identifiers with type nat get substituted at runtime. *)
+Inductive store_split (Ξ : symbols) : store -> Gamma -> Prop :=
+| TemptyΔ : forall (Γ : Gamma), interfaces Ξ = Some Γ -> store_split Ξ sNil Γ
+| Tref1ℕ : forall (Γ : Gamma) (Δ : store) (x : vart) (ℓ : loc),
+    store_split Ξ Δ Γ ->
+    store_split Ξ (x ↦ (ℓ ⋅ ◻) ◘ Δ) (x ↦ (Texpr Tptr) ◘ Γ)
+| Tref1ℕpoison : forall (Γ : Gamma) (Δ : store) (x : vart) (ℓ : loc),
+    store_split Ξ Δ Γ ->
+    store_split Ξ (x ↦ (ℓ ⋅ ☣) ◘ Δ) (x ↦ (Texpr Twptr) ◘ Γ)
+| Tsplitign : forall (Γ : Gamma) (Δ : store) (x : vart) (τ0 τ1 : ty),
+    store_split Ξ Δ Γ ->
+    store_split Ξ Δ (x ↦ (Tectx(Tarrow τ0 τ1)) ◘ Γ)
+.
+Inductive state_split : state -> Gamma -> Prop :=
+| TΩ : forall F Ξ ξ K H Δ (Γ : Gamma), store_split Ξ Δ Γ -> state_split (F ; Ξ ; ξ ; K ; H ; Δ) Γ
+.
+Inductive rt_check : state -> expr -> Ty -> Prop :=
+| Trtcheck : forall (Ω : state) (e : expr) (τ : Ty) (Γ : Gamma),
+    state_split Ω Γ ->
+    (check Γ e τ) ->
+    rt_check Ω e τ
+.
+Definition ectx_rt_check (Ω : state) (K : evalctx) (τ τ' : Ty) :=
+  forall (e : expr), rt_check Ω e τ' -> rt_check Ω (insert K e) τ
+.
+Lemma rt_check_recompose (Ω : state) (K : evalctx) (e : expr) (τ : Ty) :
+  rt_check Ω (insert K e) τ ->
+  exists τ', ectx_rt_check Ω K τ' τ /\ rt_check Ω e τ'
+.
+Proof.
+  intros H.
+  remember (insert K e).
+  destruct H.
+  induction H0.
+  - induction K; cbn in *; try congruence; subst.
+    exists τ; split; try easy; econstructor; eauto; econstructor; eauto.
+  - induction K; cbn in *; try congruence; subst.
+    exists Tℕ; split; try easy; econstructor; eauto; econstructor; eauto.
+  - induction K; cbn in *; try congruence; subst; exists Tℕ.
+    + split; try easy; econstructor; eauto; econstructor; eauto.
+    + split; inv Heqe0.
+      * econstructor; eauto. econstructor; eauto.
+Admitted.
+Lemma rt_check_decompose (Ω : state) (K : evalctx) (e : expr) (τ τ' : Ty) :
+  ectx_rt_check Ω K τ' τ ->
+  rt_check Ω e τ' ->
+  rt_check Ω (insert K e) τ
+.
+Proof. Admitted.
+
+Lemma substi Γ e x y t :
+  check Γ e t ->
+  check (substτ Γ x y) (subst x e (Fvar y)) t
+.
+Proof.
+Admitted.
+
+
+Lemma pstep_preservation Ω e τ Ω' e' a :
+  rt_check Ω e τ ->
+  Ω ▷ e --[, a ]--> Ω' ▷ e' ->
+  rt_check Ω' e' τ
+.
+Proof. Admitted.
+Lemma estep_preservation Ω e τ Ω' e' a :
+  rt_check Ω e τ ->
+  Ω ▷ e ==[, a ]==> Ω' ▷ e' ->
+  rt_check Ω' e' τ
+.
+Proof. Admitted.
+
+Lemma δ_of_Δ_poison_eq (Δ1 Δ2 : store) (x : vart) (ℓ : loc) :
+  δ_of_Δ (Δ1 ◘ x ↦ (ℓ, ◻) ◘ Δ2) = δ_of_Δ (Δ1 ◘ x ↦ (ℓ, ☣) ◘ Δ2)
+.
+Proof.
+  induction Δ1; cbn; eauto; destruct b as [[] _]; fold (append Δ1 (x ↦ (ℓ, ◻) ◘ Δ2));
+  fold (append Δ1 (x ↦ (ℓ, ☣) ◘ Δ2)); now f_equal.
+Qed.
+
+Lemma store_agree_split T__TMS Δ1 x ℓ ρ Δ2 δ :
+  store_agree δ T__TMS (Δ1 ◘ x ↦ (addr ℓ, ρ) ◘ Δ2) ->
+  exists T__TMS1 T__TMS2 ℓ', store_agree δ T__TMS1 Δ1 /\
+                    store_agree δ T__TMS2 Δ2 /\
+                    store_agree δ ({ℓ'} ∪ (TMMon.emptytmsmon)) (x ↦ (addr ℓ, ρ) ◘ sNil) /\
+                    T__TMS = TMMon.append T__TMS1 (TMMon.append ({ℓ'} ∪ TMMon.emptytmsmon) T__TMS2)
+.
+Proof.
+  induction Δ1; intros H; cbn in *.
+  - exists TMMon.emptytmsmon. exists T__TMS. exists (TMMon.addr ℓ).
+Admitted.
+
+Lemma store_agree_rsplit T__TMS1 T__TMS2 Δ1 Δ2 δ:
+  store_agree δ T__TMS1 Δ1 ->
+  store_agree δ T__TMS2 Δ2 ->
+  store_agree δ (TMMon.append T__TMS1 T__TMS2) (Δ1 ◘ Δ2)
+.
+Proof.
+Admitted.
+
+Lemma store_split_poisoned Ξ Δ1 x ℓ Δ2 Γ :
+  store_split Ξ (Δ1 ◘ x ↦ (addr ℓ, ☣) ◘ Δ2) Γ ->
+  store_split Ξ (Δ1 ◘ Δ2) Γ /\ (~ List.In x (dom Γ))
+.
+Proof. Admitted.
+Lemma store_agree_subsets δ δ' T__TMS Δ :
+  store_agree δ T__TMS Δ ->
+  MSubset δ δ' ->
+  store_agree δ' T__TMS Δ
+.
+Proof.
+  induction 1; cbn; intros Ha; eauto. constructor.
+Admitted.
+Lemma store_agree_notin_propagates ℓ (Δ : store) T__TMS :
+  ~ In (addr ℓ) (dom(δ_of_Δ Δ)) ->
+  store_agree (δ_of_Δ Δ) T__TMS Δ ->
+  TMMon.addr(ℓ) ∉ T__TMS
+.
+Proof. Admitted.
+
+Lemma base_tms_via_monitor (Ω Ω' : state) (e e' : expr) (τ : Ty) (a : event)
+                           (T__TMS : TMMon.TMSMonitor) (δ : deltamap) :
+  rt_check Ω e τ ->
+  (Ω ▷ e --[ a ]--> Ω' ▷ e') ->
+  state_agree δ T__TMS Ω ->
+  δ = δ_of_Δ (let '(_,_,_,_,Δ) := Ω in Δ) ->
+  exists (b : TMMon.event) (δ' : deltamap) (T__TMS' : TMMon.TMSMonitor),
+    MSubset δ δ'
+  /\ ev_eq δ' (msev_of_ev a) (Some b)
+  /\ (TMMon.step T__TMS (Some b) T__TMS')
+  /\ state_agree δ' T__TMS' Ω'
+  /\ (δ' = δ_of_Δ (let '(_,_,_,_,Δ) := Ω' in Δ))
+.
+Proof.
+  (*FIXME: proof is broken*)
+  (*
+  intros Aa Ab Ac Ad. inv Ab.
+  - inv Ac. assert (H3':=H3); apply store_agree_split in H3 as [T__TMS1 [T__TMS2 [ℓ__TMS [Ac1 [Ac2 [Ac3 Ac4]]]]]].
+    exists (TMMon.Suse ℓ__TMS). exists (δ_of_Δ(Δ1 ◘ x ↦ (addr ℓ, ρ) ◘ Δ2)). exists T__TMS; repeat split; try easy; try now constructor.
+    cbn. inv Ac3; eauto.  constructor; eauto. constructor; eauto. inv H7.
+    constructor; eauto. inv Ac4; easy.
+  - inv Ac. assert (H3':=H3); apply store_agree_split in H3 as [T__TMS1 [T__TMS2 [ℓ__TMS [Ac1 [Ac2 [Ac3 Ac4]]]]]].
+    exists (TMMon.Suse ℓ__TMS). exists (δ_of_Δ(Δ1 ◘ x ↦ (addr ℓ, ρ) ◘ Δ2)). exists T__TMS; repeat split; try easy; try now constructor.
+    cbn. inv Ac3; eauto.  constructor; eauto. constructor; eauto. inv H7.
+    constructor; eauto. inv Ac4; easy.
+  - inv Ac; assert (H3':=H3); apply store_agree_split in H3 as [T__TMS1 [T__TMS2 [ℓ__TMS [Ac1 [Ac2 [Ac3 Ac4]]]]]].
+    exists (TMMon.Sdealloc ℓ__TMS). exists (δ_of_Δ(Δ1 ◘ x ↦ (addr ℓ, ρ) ◘ Δ2)).
+    inv Ac3.
+    + (* Rule Cons-Agree *)
+      exists (TMMon.append T__TMS1 T__TMS2); repeat split; try easy; try now econstructor.
+      constructor; eauto using TMMon.remove_loc_from_union.
+      cbn. apply store_agree_rsplit; eauto. econstructor; eauto. cbn.
+      apply δ_of_Δ_poison_eq.
+    + (* Rule Cons-Agree-Ignore *)
+      inv Aa. inv H0. eapply store_split_poisoned in H12 as [H12a H12b].
+      inv H1; exfalso; revert H12b; clear; intros H; apply H; clear H.
+      induction Γ1; cbn; eauto.
+  - remember (TMMon.addr(Fresh.fresh F)) as ℓ__TMS;
+    remember (addr(Fresh.fresh F)) as ℓ.
+    exists (TMMon.Salloc ℓ__TMS); exists (δ_of_Δ Δ'); exists ({ℓ__TMS} ∪ T__TMS); repeat split.
+    + unfold spush in H9.
+      change ((fun Δ__y : option store => match Δ__y with
+                                     | Some Δ__y' => Some Δ__y'
+                                     | None => None
+                                     end = Some Δ') (sundup (freshv(advance F) ↦ (ℓ, ◻) ◘ Δ))) in H9.
+      destruct (option_dec (sundup ((freshv(advance F)) ↦ (ℓ, ◻) ◘ Δ))) as [Hx|Hy].
+      * apply not_eq_None_Some in Hx as [Δ__x Hx]. rewrite Hx in H9. inv H9.
+        rewrite <- (sundup_refl (freshv(advance F) ↦ (addr(fresh F), ◻) ◘ Δ) Hx).
+        rewrite <- (sundup_refl (freshv(advance F) ↦ (addr(fresh F), ◻) ◘ Δ) Hx) in Hx.
+        apply snodupinv_equiv_sundup in Hx as Hx'; assert (Hx'':=Hx'). inv Hx'.
+        remember (freshv(advance F)↦(addr(fresh F),◻)◘Δ) as Δ__s'.
+        assert (Some Δ__s' = spush (freshv(advance F)) (addr(fresh F),◻) Δ).
+        unfold spush. symmetry.
+        change ((fun Δ__y : option store => match Δ__y with
+                                      | Some Δ__y' => Some Δ__y'
+                                      | None => None
+                                      end = Some Δ__s') (sundup((freshv(advance F))↦(addr(fresh F), ◻) ◘ Δ))).
+        rewrite HeqΔ__s' in Hx; rewrite Hx. now subst.
+        eapply spush_msubset in H0. subst. now apply δΔ_msubset_invariant.
+      * now rewrite Hy in H9.
+    + inv H9. inv Ac. apply spush_ok in H1 as H1'.
+      apply snodupinv_implies_δnodupinv in H1'.
+      constructor; eauto.
+      unfold spush in H1.
+      destruct (option_dec (sundup (freshv(advance F) ↦ (addr (fresh F), ◻) ◘ Δ))) as [Hx|Hy].
+      * apply not_eq_None_Some in Hx as [Δ__x Hx]. rewrite <- (sundup_refl _ Hx) in Hx.
+        change ((fun Δ__y : option store => match Δ__y with
+                                | Some Δ'0 => Some Δ'0
+                                | None => None
+                                end = Some Δ') (sundup (freshv(advance F) ↦ (addr(fresh F), ◻) ◘ Δ))) in H1.
+        rewrite Hx in H1.
+        inv H1. cbn. now rewrite Nat.eqb_refl.
+      * change ((fun Δ__y : option store => match Δ__y with
+                                       | Some Δ'0 => Some Δ'0
+                                       | None => None
+                                       end = Some Δ') (sundup (freshv(advance F) ↦ (addr(fresh F), ◻) ◘ Δ))) in H1.
+        rewrite Hy in H1; congruence.
+    + constructor; try easy. inv Ac. apply spush_ok in H9 as H9'.
+      unfold spush in H9.
+      destruct (option_dec (sundup (freshv(advance F) ↦ (addr (fresh F), ◻) ◘ Δ))) as [Hx|Hy].
+      * apply not_eq_None_Some in Hx as [Δ__x Hx].
+        change ((fun Δ__s : option store => match Δ__s with
+                                       | Some Δ__t => Some Δ__t
+                                       | None => None
+                                       end = Some Δ') (sundup (freshv(advance F) ↦ (addr(fresh F), ◻) ◘ Δ))) in H9.
+        rewrite Hx in H9. rewrite <- Hx in H9.
+        rewrite <- (sundup_refl (freshv(advance F) ↦ (addr(fresh F), ◻) ◘ Δ)) in H9'; eauto.
+        inv H9'. eauto using store_agree_notin_propagates.
+      * change ((fun Δ__y : option store => match Δ__y with
+                                       | Some Δ'0 => Some Δ'0
+                                       | None => None
+                                       end = Some Δ') (sundup (freshv(advance F) ↦ (addr(fresh F), ◻) ◘ Δ))) in H9.
+        rewrite Hy in H9; congruence.
+    + unfold spush in H9.
+      change ((fun Δ'0 => match Δ'0 with
+                      | Some Δ'1 => Some Δ'1
+                      | None => None
+                      end = Some Δ') (sundup (freshv (advance F) ↦ (ℓ, ◻) ◘ Δ))) in H9.
+      destruct (option_dec (sundup (freshv (advance F) ↦ (ℓ, ◻) ◘ Δ))) as [Hx|Hy]; try (rewrite Hy in H9; cbn in H9; congruence).
+      apply not_eq_None_Some in Hx as [Δ__x Hx].
+      rewrite <- (sundup_refl (freshv (advance F) ↦ (ℓ, ◻) ◘ Δ) Hx) in Hx.
+      rewrite Hx in H9. inv H9.
+      econstructor; eauto.
+      * apply snodupinv_equiv_sundup in Hx as Hx'; now apply snodupinv_implies_δnodupinv in Hx'.
+      * cbn; now rewrite Nat.eqb_refl.
+      * inv Ac. apply snodupinv_equiv_sundup in Hx. inv Hx. eauto using store_agree_notin_propagates.
+      * inv Ac. cbn. eapply store_agree_subsets; try exact H3.
+        eapply cons_msubset; symmetry.
+        eapply snodupinv_equiv_sundup in Hx as Hx'; eapply snodupinv_implies_δnodupinv in Hx'.
+        eapply push_ko; cbn in Hx'; inv Hx'; auto.
+  *)
+Admitted.
+
+Lemma ctx_tms_via_monitor (Ω Ω' : state) (e e' : expr) (τ : Ty) (a : event)
+                          (T__TMS : TMMon.TMSMonitor) (δ : deltamap) :
+  rt_check Ω e τ ->
+  (Ω ▷ e ==[ a ]==> Ω' ▷ e') ->
+  state_agree δ T__TMS Ω ->
+  δ = δ_of_Δ (let '(_,_,_,_,_,Δ) := Ω in Δ) ->
+  exists (b : option TMMon.event) (δ' : deltamap) (T__TMS' : TMMon.TMSMonitor),
+     MSubset δ δ'
+  /\ (ev_eq δ' (msev_of_ev a) b)
+  /\ (TMMon.step T__TMS b T__TMS')
+  /\ state_agree δ' T__TMS' Ω'
+  /\ (δ' = δ_of_Δ (let '(_,_,_,_,_,Δ) := Ω' in Δ))
+.
+Proof.
+  intros Aa Ab Ac Ad.
+  inv Ab.
+  - eapply rt_check_recompose in Aa as [τ' [Aa0 Aa1]]. destruct Ω as [[[[[]]]]]. rename s0 into Δ.
+    eapply base_tms_via_monitor in H7; eauto.
+    deex. destruct H7 as [H7a [H7b [H7c [H7d H7e]]]].
+    destruct Ω' as [[[[[]]]]]; rename s1 into Δ'.
+    do 3 eexists; repeat split; subst; eauto.
+    now inv H7d.
+  - exists None. exists (δ_of_Δ Δ). exists T__TMS. repeat split; eauto; try easy. cbn. constructor. inv Ac. inv H4; easy. constructor. now inv Ac.
+  - inv H6; exists None; exists (δ_of_Δ Δ); exists T__TMS; repeat split; eauto; try easy; cbn; try constructor.
+    inv Ac. inv H5; easy. now inv Ac. inv Ac. inv H5; easy. now inv Ac.
+  - inv H4; exists None; exists (δ_of_Δ Δ); exists T__TMS; repeat split; eauto; try easy; cbn; try constructor.
+    inv Ac. inv H3; easy. now inv Ac. inv Ac. inv H3; easy. now inv Ac.
+  - exists None. exists (δ_of_Δ Δ). exists T__TMS. repeat split; eauto; try easy. cbn. constructor. inv Ac. inv H3; easy. constructor. now inv Ac.
+Qed.
+
+Lemma ctx_tms_via_monitor_ignore (Ω Ω' : state) (e e' : expr) (τ : Ty)
+                                 (T__TMS : TMMon.TMSMonitor) (δ : deltamap) :
+  rt_check Ω e τ ->
+  (Ω ▷ e ==[]==> Ω' ▷ e') ->
+  state_agree δ T__TMS Ω ->
+  δ = δ_of_Δ (let '(_,_,_,_,_,Δ) := Ω in Δ) ->
+  exists (δ' : deltamap) (T__TMS' : TMMon.TMSMonitor),
+     MSubset δ δ'
+  /\ (TMMon.step T__TMS None T__TMS')
+  /\ state_agree δ' T__TMS' Ω'
+  /\ (δ' = δ_of_Δ (let '(_,_,_,_,_,Δ) := Ω' in Δ))
+.
+Proof.
+  intros Aa Ab Ac Ad; destruct Ω as [[[[[]]]]]; rename s0 into Δ.
+  exists (δ_of_Δ Δ). exists T__TMS. repeat split; subst; eauto; try easy. constructor.
+  all: inv Ab; try inv H7; try easy.
+  all: inv Ac; now constructor.
+Qed.
+
+Lemma steps_tms_via_monitor (Ω Ω' : state) (e e' : expr) (τ : Ty) (As : tracepref)
+                          (T__TMS : TMMon.TMSMonitor) (δ : deltamap) :
+  rt_check Ω e τ ->
+  (Ω ▷ e ==[ As ]==>* Ω' ▷ e') ->
+  state_agree δ T__TMS Ω ->
+  δ = δ_of_Δ (let '(_,_,_,_,_,Δ) := Ω in Δ) ->
+  exists (Bs : TMMonM.tracepref) (δ' : deltamap) (T__TMS' : TMMon.TMSMonitor),
+     MSubset δ δ'
+  /\ (mstracepref_eq δ' (mstracepref_of_tracepref As) Bs)
+  /\ (TMMonM.star_step T__TMS Bs T__TMS')
+  /\ state_agree δ' T__TMS' Ω'
+  /\ (δ' = δ_of_Δ (let '(_,_,_,_,_,Δ) := Ω' in Δ))
+.
+Proof.
+  intros Aa Ab; revert δ T__TMS; dependent induction Ab; intros δ T__TMS Ac Ad.
+  - (* refl *)
+    exists (nil). exists δ. exists T__TMS. repeat split; try easy; constructor; try easy. inv Ac. now inv H1.
+  - (* trans *)
+    destruct r2 as [[Ω2|] e2]; cbn in H0; try contradiction; clear H0.
+    eapply estep_preservation in Aa as Aa'; eauto.
+    eapply ctx_tms_via_monitor in Aa as Aa''; eauto; deex; try destruct Aa'' as [Ha [Hb [Hc [Hd He]]]].
+    specialize (IHAb Ω2 Ω' e2 e' Aa' JMeq_refl JMeq_refl δ' T__TMS' Hd He).
+    deex; rename T__TMS'0 into T__TMS''; rename δ'0 into δ''; destruct IHAb as [IHAb1 [IHAb2 [IHAb3 [IHAb4 IHAb5]]]].
+    subst. destruct Ω as [[[[[]]]]]; rename s0 into Δ. destruct Ω' as [[[[[]]]]]; rename s1 into Δ'.
+    destruct Ω2 as [[[[[]]]]]; rename s2 into Δ2.
+    destruct a; cbn in Hb; inv Hb;
+    match goal with
+    | [H: TMMon.step ?T__TMS (Some(?ev)) ?T__TMS' |- _] =>
+      exists (ev :: Bs); exists (δ_of_Δ Δ'); exists T__TMS''; repeat split; eauto;
+     (try (etransitivity; eauto)); (try econstructor); eauto; (try econstructor); try eapply mget_subset; eauto
+    | [H: TMMon.step ?T__TMS None ?T__TMS' |- _] =>
+      exists Bs; exists (δ_of_Δ Δ'); exists T__TMS''; repeat split; eauto;
+      (try econstructor); eauto; (try econstructor); try eapply mget_subset; eauto
+    end;
+    repeat match goal with
+    | [H: state_agree ?δ _ _ |- Util.nodupinv ?δ] => inv H
+    | [H: store_agree ?δ _ _ |- Util.nodupinv ?δ] => inv H; eauto
+    | [H: store_agree ?δ _ _ |- state_agree ?δ _ _] => inv H; eauto
+    end; (repeat now inv IHAb4); etransitivity; eauto.
+  - (* unimp *)
+    destruct r2 as [[Ω2|] e2]; cbn in H0; try contradiction; clear H0.
+    eapply estep_preservation in Aa as Aa'; eauto.
+    eapply ctx_tms_via_monitor_ignore in Aa as Aa''; eauto; deex; destruct Aa'' as [Ha [Hb [Hc Hd]]].
+    specialize (IHAb Ω2 Ω' e2 e' Aa' JMeq_refl JMeq_refl δ' T__TMS' Hc Hd).
+    destruct Ω as [[[[[]]]]]; rename s0 into Δ; destruct Ω2 as [[[[[]]]]]; rename s1 into Δ2.
+    deex; rename T__TMS'0 into T__TMS''; rename δ'0 into δ''; destruct IHAb as [IHAb1 [IHAb2 [IHAb3 [IHAb4 IHAb5]]]].
+    destruct Ω' as [[[[[]]]]]; rename s2 into Δ'; subst.
+    exists Bs. exists (δ_of_Δ Δ'). exists T__TMS''. repeat split; eauto.
+    + etransitivity; eauto.
+    + econstructor; eauto; econstructor; eapply mget_subset; eauto.
+    + now inv IHAb4.
+Qed.
+
+Lemma toplevel_check_weakening Ξ Γ foo τ0 τ1 bar τ0' τ1' x e__bar :
+  interfaces (bar ↦ (x, Tectx(Tarrow τ0' τ1'), e__bar) ◘ Ξ) = Some Γ ->
+  mget Γ foo = Some(Tectx(Tarrow τ0 τ1)) ->
+  NoOwnedPtr Γ ->
+  foo <> bar ->
+  check (bar ↦ (Tectx(Tarrow τ0' τ1')) ◘ Γ) (Fvar foo) (Tarrow τ0 τ1) ->
+  check Γ (Fvar foo) (Tarrow τ0 τ1)
+.
+Proof.
+Admitted.
+
+Theorem s_is_tms (Ξ : symbols) (ξ : commlib) As Ω f :
+  wstep (Cprog Ξ ξ) As (Ω ▷ (Xres f)) ->
+  TMS As.
+Proof.
+  intros Ha; inv Ha; unfold prog_check in H1.
+  destruct (option_dec (interfaces Ξ)) as [Hx|Hx]; try (rewrite Hx in H0; contradiction).
+  apply not_eq_None_Some in Hx as [x__x Hx]; rewrite Hx in H1.
+  remember (Fresh.empty_fresh ; Ξ ; nil ; nil ; hNil ; sNil) as Ω__init; pose ((mapNil _ _) : deltamap) as δ__init.
+  assert (state_agree (mapNil _ _) TMMon.emptytmsmon Ω__init) by (subst; repeat constructor).
+  assert (δ__init= δ_of_Δ (let '(_,_,_,_,_,Δ) := Ω__init in Δ)) by (subst; cbn; easy).
+  subst. eapply steps_tms_via_monitor in H4; eauto.
+  deex; destruct H4 as [F__a [F__b [F__c [F__d F__e]]]].
+  intros MAs H__As. exists δ'. exists Bs. split; subst. exact F__b.
+  unfold TMMon.TMS. exists T__TMS'; try eexact F__c.
+  econstructor. repeat constructor. exact Hx.
+  econstructor. instantiate (1:=Tℕ); constructor.
+  instantiate (1:=Tℕ); constructor.
+  shelve.
+  constructor.
+  option_boilerplate (mget x__x "main"%string); rewrite Hx0 in H1; try easy.
+  destruct x; try easy; destruct e; try easy; destruct t, t0; try easy.
+  crush_noownedptrf x__x. now apply noownedptr_equiv_noownedptrf.
+  now rewrite Hx2 in H1. constructor; now inv H.
+  now rewrite Hx in H1.
+  Unshelve.
+  option_boilerplate (mget x__x "main"%string); rewrite Hx0 in H1; try easy.
+  destruct x; try easy; destruct e; try easy; destruct t, t0; try easy.
+  crush_noownedptrf x__x; try now rewrite Hx2 in H1.
+  clear H H4 H0 Hx1 δ__init; revert x__x H1 Hx Hx0 Hx2; induction Ξ; intros.
+  - inv Hx; inv Hx0.
+  - destruct b; destruct p. destruct t; try inv H1. destruct e0. destruct H1 as [H1__a [H1__b [H1__c H1__d]]].
+    destruct (eq_dec a "main"%string).
+    + subst. cbn in Hx.
+      option_boilerplate (interfaces Ξ); rewrite Hx1 in Hx; try easy.
+      inv Hx. change (check (mapNil _ _ ◘ "main"%string ↦ Tectx(Tarrow t t0) ◘ x0) (Fvar "main"%string) (Tectx(Tarrow Tℕ Tℕ))).
+      cbn in Hx0; inv Hx0. eapply CTvar.
+      admit.
+      easy. easy. apply noownedptr_equiv_noownedptrf in Hx2.
+      change (NoOwnedPtr ("main"%string ↦ Tectx(Tarrow Tℕ Tℕ) ◘ mapNil _ _ ◘ x0)) in Hx2.
+      now apply noownedptr_split in Hx2 as [Hx2__a Hx2__b].
+    + (*indu is bonkers*) admit.
+Admitted.
